theories/stacked_borrows/heap.v
@@ -95,7 +95,8 @@ Definition state_upd_mem (f : mem → mem) σ :=
   mkState (f σ.(shp)) σ.(sst) σ.(scs) σ.(snp) σ.(snc).
 Definition state_upd_stacks (f : stacks → stacks) σ :=
   mkState σ.(shp) (f σ.(sst)) σ.(scs) σ.(snp) σ.(snc).
-
+Definition state_upd_calls (f : call_id_set → call_id_set) σ :=
+  mkState σ.(shp) σ.(sst) (f σ.(scs)) σ.(snp) σ.(snc).
 
 
 (* maintain for each tag: the permissions (public or unique) and, optionally, the
@@ -136,6 +137,11 @@ Section mem_bijection.
      TODO: can we make that more beautiful? all the different invariants are interleaved in subtle ways, which makes modular reasoning really hard... *)
     Context (M_tag : gmap ptr_id (tag_kind * unit)) (M_t M_s : gmap (ptr_id * loc) scalar) (Mcall_t : gmap call_id (gmap ptr_id (gset loc))).
 
+
+    Definition call_set_in (M : gmap ptr_id (gset loc)) t l :=
+      ∃ L, M !! t = Some L ∧ l ∈ L.
+    Definition call_set_in' (M : gmap call_id (gmap ptr_id (gset loc))) c t l :=
+      ∃ M', M !! c = Some M' ∧ call_set_in M' t l.
     Definition pub_loc σ_t σ_s (l : loc) : iProp Σ :=
       ∀ sc_t, ⌜σ_t.(shp) !! l = Some sc_t⌝ → ∃ sc_s, ⌜σ_s.(shp) !! l = Some sc_s⌝ ∗ sc_rel sc_t sc_s.
     Definition priv_loc t (l : loc) : Prop :=
@@ -143,7 +149,7 @@ Section mem_bijection.
         (* local *)
         (tk = tk_local ∨
         (* unique with protector *)
-        (tk = tk_unq ∧ ∃ c M' L, Mcall_t !! c = Some M' ∧ M' !! t = Some L ∧ l ∈ L)).
+        (tk = tk_unq ∧ ∃ c, call_set_in' Mcall_t c t l)).
 
     (* This definition enforces quite strict requirements on the state:
       - the domains of the heaps shp are the same
@@ -177,7 +183,7 @@ Section bijection_lemmas.
   Local Notation state_rel := (state_rel sc_rel).
 
   Lemma state_rel_get_pure Mtag Mt Mcall σ_t σ_s :
-    state_rel Mtag Mt Mcall σ_t σ_s -∗ ⌜σ_s.(snp) = σ_t.(snp) ∧ σ_s.(snc) = σ_t.(snc) ∧ σ_s.(scs) = σ_t.(scs)⌝.
+    state_rel Mtag Mt Mcall σ_t σ_s -∗ ⌜σ_s.(sst) = σ_t.(sst) ∧ σ_s.(snp) = σ_t.(snp) ∧ σ_s.(snc) = σ_t.(snc) ∧ σ_s.(scs) = σ_t.(scs)⌝.
   Proof. iIntros "(% & % & % & % & % & ?)". eauto. Qed.
   Lemma state_rel_stacks_eq Mtag Mt Mcall σ_t σ_s :
     state_rel Mtag Mt Mcall σ_t σ_s -∗ ⌜σ_s.(sst) = σ_t.(sst)⌝.
@@ -318,25 +324,39 @@ Section call_defs.
       c ∈ σ.(scs) ∧
       (* for every ptr_id *)
       ∀ pid (S : gset loc), M' !! pid = Some S →
-        pid < σ.(snp) ∧
+        (pid < σ.(snp))%nat ∧
         (* for every protected location [l], there needs to be a protector in the stack *)
         ∀ (l : loc), l ∈ S → ∃ s pm, σ.(sst) !! l = Some s ∧
           mkItem pm (Tagged pid) (Some c) ∈ s ∧ pm ≠ Disabled.
 
-  Definition call_set_in' (M : gmap call_id (gmap ptr_id (gset loc))) c t l :=
-    ∃ M' L, M !! c = Some M' ∧ M' !! t = Some L ∧ l ∈ L.
-  Definition call_set_in (M : gmap ptr_id (gset loc)) t l :=
-    ∃ L, M !! t = Some L ∧ l ∈ L.
+  Definition loc_protected_by σ t l c :=
+    c ∈ σ.(scs) ∧ (t < σ.(snp))%nat ∧ ∃ stk pm, σ.(sst) !! l = Some stk ∧
+      mkItem pm (Tagged t) (Some c) ∈ stk ∧ pm ≠ Disabled.
   Lemma call_set_interp_access M σ c t l :
     call_set_interp M σ →
     call_set_in' M c t l →
-    c ∈ σ.(scs) ∧ t < σ.(snp) ∧ ∃ stk pm, σ.(sst) !! l = Some stk ∧
-      mkItem pm (Tagged t) (Some c) ∈ stk ∧ pm ≠ Disabled.
+    loc_protected_by σ t l c.
   Proof.
-    intros Hinterp (M' & L & HM_some & HM'_some & Hin).
+    intros Hinterp (M' & HM_some & L & HM'_some & Hin).
     specialize (Hinterp _ _ HM_some) as (? & Hinterp).
     specialize (Hinterp _ _ HM'_some) as (? & Hinterp).
     specialize (Hinterp _ Hin). done.
+  Qed.
+
+  Lemma call_set_interp_remove c M σ :
+    call_set_interp M σ →
+    call_set_interp (delete c M) (state_upd_calls (.∖ {[c]}) σ).
+  Proof.
+    intros Hinterp c' M' Hsome. destruct (decide (c' = c)) as [-> | Hneq].
+    { rewrite lookup_delete in Hsome. done. }
+    rewrite lookup_delete_ne in Hsome; last done.
+    apply Hinterp in Hsome as (Hin & Hpid).
+    split.
+    { destruct σ; cbn in *. apply elem_of_difference; split; first done. by apply not_elem_of_singleton. }
+    intros t S HS.
+    apply Hpid in HS as (Ht & Hlookup). split; first by destruct σ.
+    intros l Hl. apply Hlookup in Hl as (s & pm & Hsst & Hs & Hpm).
+    exists s, pm. split_and!; [ | done..]. by destruct σ.
   Qed.
 
 End call_defs.
@@ -361,6 +381,12 @@ Section heap_defs.
         mkItem pm (Tagged t) pro ∈ st ∧ pm ≠ Disabled
     end.
 
+  Lemma loc_protected_bor_state_pre l t c σ tk :
+    loc_protected_by σ t l c → bor_state_pre l t tk σ.
+  Proof.
+    intros (_ & _ & (stk & pm & ?)). destruct tk; [| | done]; rewrite /bor_state_pre; eauto.
+  Qed.
+
   Definition bor_state_own (l : loc) (t : ptr_id) (tk : tag_kind) (σ : state) :=
     match tk with
     | tk_local => σ.(sst) !! l = Some ([mkItem Unique (Tagged t) None])
@@ -368,6 +394,10 @@ Section heap_defs.
         st = mkItem Unique (Tagged t) opro :: st'
     | tk_pub => ∃ st, σ.(sst) !! l = Some st ∧ t ∈ active_SRO st
     end.
+
+  Lemma bor_state_own_some_stack l t tk σ :
+    bor_state_own l t tk σ → ∃ stk, σ.(sst) !! l = Some stk.
+  Proof. rewrite /bor_state_own. destruct tk; naive_solver. Qed.
 
   Definition loc_controlled (l : loc) (t : ptr_id) (tk : tag_kind) (sc : scalar) (σ : state) :=
     (bor_state_pre l t tk σ → bor_state_own l t tk σ ∧ σ.(shp) !! l = Some sc).
@@ -528,30 +558,41 @@ Section heap_defs.
   Proof. intros Hag Hsome. apply Hag, Hsome. Qed.
 
   Definition tag_interp (M : gmap ptr_id (tag_kind * unit)) (M_t M_s : gmap (ptr_id * loc) scalar) σ_t σ_s : Prop :=
-    ∀ (t : ptr_id) tk, M !! t = Some (tk, ()) →
+    (∀ (t : ptr_id) tk, M !! t = Some (tk, ()) →
       (* tags are valid *)
       (t < σ_t.(snp))%nat ∧ (t < σ_s.(snp))%nat ∧
       (* at all locations, the values agree, and match the physical state assuming the tag currently has control over the location *)
       (∀ l sc_t, M_t !! (t, l) = Some sc_t → loc_controlled l t tk sc_t σ_t) ∧
       (∀ l sc_s, M_s !! (t, l) = Some sc_s → loc_controlled l t tk sc_s σ_s) ∧
-      dom_agree_on_tag M_t M_s t.
+      dom_agree_on_tag M_t M_s t) ∧
+    (∀ (t : ptr_id) (l : loc), is_Some (M_t !! (t, l)) → is_Some (M !! t)) ∧
+    (∀ (t : ptr_id) (l : loc), is_Some (M_s !! (t, l)) → is_Some (M !! t)).
 End heap_defs.
 
 
 Notation "p '$$' tk" := (tkmap_elem tag_name p tk ()) (at level 50).
 
-Notation "l '↦t[unq]{' t } sc" := (ghost_map_elem heap_view_target_name (t, l) (DfracOwn 1) sc)
-  (at level 20, format "l  ↦t[unq]{ t }  sc") : bi_scope.
-Notation "l '↦s[unq]{' t } sc" := (ghost_map_elem heap_view_source_name (t, l) (DfracOwn 1) sc)
-  (at level 20, format "l  ↦s[unq]{ t }  sc") : bi_scope.
-Notation "l '↦t[local]{' t } sc" := (ghost_map_elem heap_view_target_name (t, l) (DfracOwn 1) sc)
-  (at level 20, format "l  ↦t[local]{ t }  sc") : bi_scope.
-Notation "l '↦s[local]{' t } sc" := (ghost_map_elem heap_view_source_name (t, l) (DfracOwn 1) sc)
-  (at level 20, format "l  ↦s[local]{ t }  sc") : bi_scope.
-Notation "l '↦t[pub]{' t } sc" := (ghost_map_elem heap_view_target_name (t, l) (DfracDiscarded) sc)
-  (at level 20, format "l  ↦t[pub]{ t }  sc") : bi_scope.
-Notation "l '↦s[pub]{' t } sc" := (ghost_map_elem heap_view_source_name (t, l) (DfracDiscarded) sc)
-  (at level 20, format "l  ↦s[pub]{ t }  sc") : bi_scope.
+Definition tk_to_frac (tk : tag_kind) :=
+  match tk with
+  | tk_pub => DfracDiscarded
+  | _ => DfracOwn 1
+  end.
+Notation "l '↦t[' tk ']{' t } sc" := (ghost_map_elem heap_view_target_name (t, l) (tk_to_frac tk) sc)
+  (at level 20, format "l  ↦t[ tk ]{ t }  sc") : bi_scope.
+Notation "l '↦s[' tk ']{' t } sc" := (ghost_map_elem heap_view_source_name (t, l) (tk_to_frac tk) sc)
+  (at level 20, format "l  ↦s[ tk ]{ t }  sc") : bi_scope.
+(*Notation "l '↦t[unq]{' t } sc" := (ghost_map_elem heap_view_target_name (t, l) (DfracOwn 1) sc)*)
+  (*(at level 20, format "l  ↦t[unq]{ t }  sc") : bi_scope.*)
+(*Notation "l '↦s[unq]{' t } sc" := (ghost_map_elem heap_view_source_name (t, l) (DfracOwn 1) sc)*)
+  (*(at level 20, format "l  ↦s[unq]{ t }  sc") : bi_scope.*)
+(*Notation "l '↦t[local]{' t } sc" := (ghost_map_elem heap_view_target_name (t, l) (DfracOwn 1) sc)*)
+  (*(at level 20, format "l  ↦t[local]{ t }  sc") : bi_scope.*)
+(*Notation "l '↦s[local]{' t } sc" := (ghost_map_elem heap_view_source_name (t, l) (DfracOwn 1) sc)*)
+  (*(at level 20, format "l  ↦s[local]{ t }  sc") : bi_scope.*)
+(*Notation "l '↦t[pub]{' t } sc" := (ghost_map_elem heap_view_target_name (t, l) (DfracDiscarded) sc)*)
+  (*(at level 20, format "l  ↦t[pub]{ t }  sc") : bi_scope.*)
+(*Notation "l '↦s[pub]{' t } sc" := (ghost_map_elem heap_view_source_name (t, l) (DfracDiscarded) sc)*)
+  (*(at level 20, format "l  ↦s[pub]{ t }  sc") : bi_scope.*)
 
 
 Section state_interp.
@@ -581,7 +622,7 @@ Section state_interp.
     ⌜state_wf σ_t⌝.
 
   Lemma bor_interp_get_pure σ_t σ_s :
-    bor_interp σ_t σ_s -∗ ⌜σ_s.(snp) = σ_t.(snp) ∧ σ_s.(snc) = σ_t.(snc) ∧ σ_s.(scs) = σ_t.(scs) ∧ state_wf σ_s ∧ state_wf σ_t⌝.
+    bor_interp σ_t σ_s -∗ ⌜σ_s.(sst) = σ_t.(sst) ∧ σ_s.(snp) = σ_t.(snp) ∧ σ_s.(snc) = σ_t.(snc) ∧ σ_s.(scs) = σ_t.(scs) ∧ state_wf σ_s ∧ state_wf σ_t⌝.
   Proof.
     iIntros "(% & % & % & % & ? & Hstate & _ & _ & % & %)".
     iPoseProof (state_rel_get_pure with "Hstate") as "%".
@@ -599,29 +640,98 @@ End state_interp.
 (** Array generalizes pointsto connectives to lists of scalars *)
 Definition array_tag `{!bor_stateG Σ} γh (t : ptr_id) (l : loc) (dq : dfrac) (scs : list scalar) : iProp Σ :=
   ([∗ list] i ↦ sc ∈ scs, ghost_map_elem γh (t, l +ₗ i) dq sc)%I.
-
-Definition tk_to_frac (tk : tag_kind) :=
-  match tk with
-  | tk_pub => DfracDiscarded
-  | _ => DfracOwn 1
-  end.
 Notation "l '↦t∗[' tk ']{' t } scs" := (array_tag heap_view_target_name t l (tk_to_frac tk) scs)
   (at level 20, format "l  ↦t∗[ tk ]{ t }  scs") : bi_scope.
 Notation "l '↦s∗[' tk ']{' t } scs" := (array_tag heap_view_source_name t l (tk_to_frac tk) scs)
   (at level 20, format "l  ↦s∗[ tk ]{ t }  scs") : bi_scope.
 
-Notation "l '↦t∗[unq]{' t } scs" := (array_tag heap_view_target_name t l (DfracOwn 1) scs)
-  (at level 20, format "l  ↦t∗[unq]{ t }  scs") : bi_scope.
-Notation "l '↦s∗[unq]{' t } scs" := (array_tag heap_view_source_name t l (DfracOwn 1) scs)
-  (at level 20, format "l  ↦s∗[unq]{ t }  scs") : bi_scope.
-Notation "l '↦t∗[local]{' t } scs" := (array_tag heap_view_target_name t l (DfracOwn 1) scs)
-  (at level 20, format "l  ↦t∗[local]{ t }  scs") : bi_scope.
-Notation "l '↦s∗[local]{' t } scs" := (array_tag heap_view_source_name t l (DfracOwn 1) scs)
-  (at level 20, format "l  ↦s∗[local]{ t }  scs") : bi_scope.
-Notation "l '↦t∗[pub]{' t } scs" := (array_tag heap_view_target_name t l (DfracDiscarded) scs)
-  (at level 20, format "l  ↦t∗[pub]{ t }  scs") : bi_scope.
-Notation "l '↦s∗[pub]{' t } scs" := (array_tag heap_view_source_name t l (DfracDiscarded) scs)
-  (at level 20, format "l  ↦s∗[pub]{ t }  scs") : bi_scope.
+Lemma ghost_map_array_tag_lookup `{!bor_stateG Σ} (γh : gname) (q : Qp) (M : gmap (ptr_id * loc) scalar) (scs : list scalar) (t : ptr_id) (l : loc) dq :
+  ghost_map_auth γh q M -∗
+  ([∗ list] i ↦ sc ∈ scs, ghost_map_elem γh (t, l +ₗ i) dq sc) -∗
+  ⌜∀ i : nat, (i < length scs)%nat → M !! (t, l +ₗ i) = scs !! i⌝.
+Proof.
+  iIntros "Hauth Helem". iInduction scs as [ |sc scs ] "IH" forall (l) "Hauth Helem".
+  - iPureIntro; cbn. lia.
+  - rewrite big_sepL_cons. iDestruct "Helem" as "[Hsc Hscs]".
+    iPoseProof (ghost_map_lookup with "Hauth Hsc") as "%Hl".
+    iDestruct ("IH" $! (l +ₗ 1) with "Hauth [Hscs]") as "%IH".
+    { iApply (big_sepL_mono with "Hscs"). intros i sc' Hs. cbn. rewrite shift_loc_assoc.
+      replace (Z.of_nat $ S i) with (1 + i)%Z by lia. done. }
+    iPureIntro. intros i Hle. destruct i; first done.
+    replace (Z.of_nat $ S i) with (1 + i)%Z by lia. cbn in *. rewrite -(IH i); last lia.
+    by rewrite shift_loc_assoc.
+Qed.
+
+Fixpoint array_tag_map (l : loc) (t : ptr_id) (v : list scalar) : gmap (ptr_id * loc) scalar :=
+  match v with
+  | [] => ∅
+  | sc :: v' => <[(t, l) := sc]> (array_tag_map (l +ₗ 1) t v')
+  end.
+Lemma array_tag_map_lookup1 l t v t' l' :
+  is_Some (array_tag_map l t v !! (t', l')) →
+  t' = t ∧ l.1 = l'.1 ∧ l.2 ≤ l'.2 < l.2 + length v.
+Proof.
+  induction v as [ | sc v IH] in l |-*.
+  - simpl. rewrite lookup_empty. intros [? [=]].
+  - simpl. move => [sc0 ]. rewrite lookup_insert_Some. move => [[[= <- <-] Heq] | [Hneq Ht]]; first lia.
+    move : (IH (l +ₗ 1) ltac:(eauto)). destruct l. simpl. lia.
+Qed.
+Lemma array_tag_map_lookup2 l t v t' l' : 
+  is_Some (array_tag_map l t v !! (t', l')) →
+  t' = t ∧ ∃ i, (i < length v)%nat ∧ l' = l +ₗ i.
+Proof. 
+  intros (-> & H1 & H2)%array_tag_map_lookup1.
+  split; first done. exists (Z.to_nat (l'.2 - l.2)). 
+  destruct l, l';  rewrite /shift_loc; simpl in *. split. 
+  - lia.
+  - apply pair_equal_spec. split; lia. 
+Qed.
+
+Lemma array_tag_map_lookup_Some l t v (i : nat) :
+  (i < length v)%nat →
+  array_tag_map l t v !! (t, l +ₗ i) = v !! i.
+Proof.
+  induction v as [ | sc v IH] in l, i |-*.
+  - simpl. lia.
+  - simpl. intros Hi. destruct i as [ | i].
+    + rewrite shift_loc_0_nat. rewrite lookup_insert. done.
+    + rewrite lookup_insert_ne; first last. { destruct l; simpl; intros [= ?]; lia. }
+      move : (IH (l +ₗ 1) i ltac:(lia)). rewrite shift_loc_assoc.
+      by replace (Z.of_nat (S i)) with (1 + i) by lia.
+Qed.
+
+Lemma ghost_map_array_tag_update `{!bor_stateG Σ} (γh : gname) (M : gmap (ptr_id * loc) scalar) (v v' : list scalar) (t : ptr_id) (l : loc) :
+  ghost_map_auth γh 1 M -∗
+  ([∗ list] i ↦ sc ∈ v, ghost_map_elem γh (t, l +ₗ i) (DfracOwn 1) sc) ==∗
+  ([∗ list] i ↦ sc' ∈ v', ghost_map_elem γh (t, l +ₗ i) (DfracOwn 1) sc') ∗
+  ghost_map_auth γh 1 (array_tag_map l t v' ∪ M).
+Proof.
+Admitted.
+
+Lemma ghost_map_array_tag_insert `{!bor_stateG Σ} (γh : gname) (M : gmap (ptr_id * loc) scalar) (v : list scalar) (t : ptr_id) (l : loc) :
+  (∀ i : nat, (i < length v)%nat → M !! (t, l +ₗ i) = None) →
+  ghost_map_auth γh 1 M  ==∗
+  ([∗ list] i ↦ sc ∈ v, ghost_map_elem γh (t, l +ₗ i) (DfracOwn 1) sc) ∗
+  ghost_map_auth γh 1 (array_tag_map l t v ∪ M).
+Proof.
+Admitted.
+
+Lemma ghost_map_array_tag_tk `{!bor_stateG Σ} (γh : gname) (v : list scalar) (t : ptr_id) (l : loc) tk :
+  ([∗ list] i ↦ sc ∈ v, ghost_map_elem γh (t, l +ₗ i) (DfracOwn 1) sc) ==∗
+  ([∗ list] i ↦ sc ∈ v, ghost_map_elem γh (t, l +ₗ i) (tk_to_frac tk) sc).
+Proof.
+  destruct tk; cbn; [ | by eauto | by eauto].
+  iInduction v as [| sc v] "IH" forall (l); first by eauto.
+  rewrite !big_sepL_cons. iIntros "[Hh Hr]".
+  iMod (ghost_map_elem_persist with "Hh") as "$".
+  iMod ("IH" $! (l +ₗ 1) with "[Hr]") as "Hr".
+  - iApply (big_sepL_mono with "Hr"). intros i sc' Hs. simpl. rewrite shift_loc_assoc.
+    by replace (Z.of_nat (S i)) with (1 + i) by lia.
+  - iModIntro.
+    iApply (big_sepL_mono with "Hr"). intros i sc' Hs. simpl. rewrite shift_loc_assoc.
+    by replace (Z.of_nat (S i)) with (1 + i) by lia.
+Qed.
+
 
 (** Lemmas / Accessors *)
 Add Printing Constructor state item.
@@ -642,8 +752,8 @@ Section lemmas.
       (mkState (init_mem l_t (tsize T) σ_t.(shp)) (init_stacks σ_t.(sst) l_t (tsize T) (Tagged σ_t.(snp))) σ_t.(scs) (S σ_t.(snp)) σ_t.(snc))
       (mkState (init_mem l_s (tsize T) σ_s.(shp)) (init_stacks σ_s.(sst) l_s (tsize T) (Tagged σ_s.(snp))) σ_s.(scs) (S σ_s.(snp)) σ_s.(snc)) ∗
       t $$ tk_local ∗
-      l_t ↦t∗[local]{t} repeat ScPoison (tsize T) ∗
-      l_s ↦s∗[local]{t} repeat ScPoison (tsize T).
+      l_t ↦t∗[tk_local]{t} repeat ScPoison (tsize T) ∗
+      l_s ↦s∗[tk_local]{t} repeat ScPoison (tsize T).
   Proof.
     iIntros "(% & % & % & % & ? & Hstate & ? & Htag & %Hwf_s & %Hwf_t)".
     (* 1. allocate new local locations
@@ -658,7 +768,7 @@ Section lemmas.
 
   Lemma state_wf_upd_mem σ l sc :
     is_Some (σ.(shp) !! l) →
-    wf_scalar σ sc →
+    wf_scalar σ.(snp) sc →
     state_wf σ →
     state_wf (state_upd_mem (<[l := sc]>) σ).
   Proof.
@@ -676,36 +786,26 @@ Section lemmas.
         eapply state_wf_mem_tag; done.
     Qed.
 
-  Lemma heap_local_access_target σ_t σ_s (t : ptr_id) l  sc :
+  Lemma heap_local_write_target σ_t σ_s (t : ptr_id) l sc sc' :
     bor_interp σ_t σ_s -∗
-    l ↦t[local]{t} sc -∗
+    l ↦t[tk_local]{t} sc -∗
     t $$ tk_local -∗
-    ⌜σ_t.(shp) !! l = Some sc⌝ ∗
-    ⌜σ_t.(sst) !! l = Some [mkItem Unique (Tagged t) None]⌝ ∗
-    ⌜wf_scalar σ_t sc⌝ ∗
-    (∀ sc',
-      ⌜wf_scalar σ_t sc'⌝ -∗
-      (*stack_wf st' σ_t -∗ *)
-      |==>
-      bor_interp (state_upd_mem (<[l := sc']>) σ_t) σ_s ∗
-      l ↦t[local]{t} sc').
+    ⌜wf_scalar σ_t.(snp) sc'⌝ ==∗
+    bor_interp (state_upd_mem (<[l := sc']>) σ_t) σ_s ∗
+    l ↦t[tk_local]{t} sc' ∗
+    t $$ tk_local.
   Proof.
     iIntros "(% & % & % & % & (Hc & Htag_auth & Htag_t_auth & Htag_s_auth) & Hsrel & ? & %Htag_interp & %Hwf_s & %Hwf_t)".
-    iIntros "Hp Htag".
+    iIntros "Hp Htag %Hwf_sc".
     iPoseProof (tkmap_lookup with "Htag_auth Htag") as "%Htag_lookup".
+    destruct Htag_interp as (Htag_interp & Ht_dom & Hs_dom).
     destruct (Htag_interp _ _ Htag_lookup) as (_ & _ & Ht & Hs & Hagree).
     iPoseProof (ghost_map_lookup with "Htag_t_auth Hp") as "%Ht_lookup".
     specialize (Ht _ _ Ht_lookup) as Hcontrol.
     specialize (loc_controlled_local _ _ _ _ Hcontrol) as (Hstack & Hmem).
-    iSplitR; first done. iSplitR; first done.
-    iSplitR. { iPureIntro. intros tg l' ->.
-      destruct tg as [tg | ]; last done.
-      eapply state_wf_mem_tag; done.
-    }
 
-    iIntros (sc') "%Hwf_sc".
     iMod (ghost_map_update sc' with "Htag_t_auth Hp") as "[Htag_t_auth $]".
-    iModIntro. rewrite /bor_interp.
+    iModIntro. iFrame "Htag". rewrite /bor_interp.
     iExists M_call, M_tag, (<[(t, l):=sc']> M_t), M_s.
     iFrame. cbn. iSplitL "Hsrel".
     { iApply (state_rel_upd_priv_target with "Hsrel").
@@ -718,112 +818,180 @@ Section lemmas.
     }
 
     iPureIntro.
-    intros t' tk' (? & ? & H')%Htag_interp. do 2 (split; first done).
-    destruct H' as (Ha_t & Ha_s & Hagree').
-    split_and!; [ | done | ].
-    - intros l' sc_t.
-      destruct (decide (t = t')) as [<- | Hneq]; first last.
-      { rewrite lookup_insert_ne; last congruence. intros Hsc_t.
-        destruct (decide (l' = l)) as [-> | Hneq_loc].
-        { (* this is fine as tag t has local ownership: t' doesn't have any control *)
-          eapply loc_controlled_local_authoritative; [ | by apply Ha_t | done].
-          eapply loc_controlled_mem_insert. done.
+    split_and!.
+    - intros t' tk' (? & ? & H')%Htag_interp. do 2 (split; first done).
+      destruct H' as (Ha_t & Ha_s & Hagree').
+      split_and!; [ | done | ].
+      + intros l' sc_t.
+        destruct (decide (t = t')) as [<- | Hneq]; first last.
+        { rewrite lookup_insert_ne; last congruence. intros Hsc_t.
+          destruct (decide (l' = l)) as [-> | Hneq_loc].
+          { (* this is fine as tag t has local ownership: t' doesn't have any control *)
+            eapply loc_controlled_local_authoritative; [ | by apply Ha_t | done].
+            eapply loc_controlled_mem_insert. done.
+          }
+          apply loc_controlled_mem_insert_ne; [done | by apply Ha_t].
         }
-        apply loc_controlled_mem_insert_ne; [done | by apply Ha_t].
-      }
-      revert Ha_t.
-      destruct (decide (l' = l)) as [-> | Hneq_loc] => Ha_t.
-      + rewrite lookup_insert => [= ->]. by eapply loc_controlled_mem_insert, Ha_t.
-      + rewrite lookup_insert_ne; last congruence. intros ?.
-        eapply loc_controlled_mem_insert_ne; [done | by apply Ha_t].
-    - destruct (decide (t = t')) as [<- | Hneq].
-      + eapply dom_agree_on_tag_upd_target; eauto.
-      + eapply dom_agree_on_tag_upd_ne_target; eauto.
+        revert Ha_t.
+        destruct (decide (l' = l)) as [-> | Hneq_loc] => Ha_t.
+        * rewrite lookup_insert => [= ->]. by eapply loc_controlled_mem_insert, Ha_t.
+        * rewrite lookup_insert_ne; last congruence. intros ?.
+          eapply loc_controlled_mem_insert_ne; [done | by apply Ha_t].
+      + destruct (decide (t = t')) as [<- | Hneq].
+        * eapply dom_agree_on_tag_upd_target; eauto.
+        * eapply dom_agree_on_tag_upd_ne_target; eauto.
+    - intros t' l'. rewrite lookup_insert_is_Some. intros [[= <- <-] | [_ ?%Ht_dom]]; last done. eauto.
+    - done.
   Qed.
 
-  Lemma heap_local_accessN_target' σ_t σ_s (t : ptr_id) l scs :
-    bor_interp σ_t σ_s -∗
-    l ↦t∗[local]{t} scs -∗
-    t $$ tk_local -∗
-    ⌜∀ i : nat, (i < length scs)%nat → σ_t.(shp) !! (l +ₗ i) = scs !! i ⌝ ∗
-    ⌜∀ i:nat, (i < length scs)%nat → σ_t.(sst) !! (l +ₗ i) = Some [mkItem Unique (Tagged t) None]⌝ ∗
-    (∀ scs',
-      ⌜length scs' = length scs⌝ -∗
-      ⌜Forall (wf_scalar σ_t) scs'⌝ -∗
-      (*stack_wf st' σ_t -∗ *)
-      |==>
-      bor_interp (state_upd_mem (λ m, heap_array l scs' ∪ m) σ_t) σ_s ∗
-      l ↦t∗[local]{t} scs').
-  Proof.
-  Admitted.
 
-  Lemma heap_local_accessN_target σ_t σ_s (t : ptr_id) l scs :
-    bor_interp σ_t σ_s -∗
-    l ↦t∗[local]{t} scs -∗
-    t $$ tk_local -∗
-    ⌜read_mem l (length scs) σ_t.(shp) = Some scs⌝ ∗
-    ⌜∀ i:nat, (i < length scs)%nat → σ_t.(sst) !! (l +ₗ i) = Some [mkItem Unique (Tagged t) None]⌝ ∗
-    ⌜scs <<t σ_t.(snp)⌝ ∗
-    (∀ scs',
-      ⌜length scs' = length scs⌝ -∗
-      ⌜scs' <<t σ_t.(snp) ⌝ -∗
-      (*stack_wf st' σ_t -∗ *)
-      |==>
-      bor_interp (state_upd_mem (write_mem l scs') σ_t) σ_s ∗
-      l ↦t∗[local]{t} scs').
+  Lemma tag_values_included_iff v t :
+    tag_values_included v t ↔ (∀ i, (i < length v)%nat → wf_scalar t (v !!! i)).
   Proof.
-  Admitted.
-
+    rewrite /tag_values_included /wf_scalar. split.
+    - intros Hin i Hi t' l Hvi. eapply (Hin l). rewrite -Hvi. by apply elem_of_list_lookup_total_2.
+    - intros Hs l tg (i & Hi & Hl)%elem_of_list_lookup_total_1. by eapply Hs.
+  Qed.
   Lemma heap_local_readN_target σ_t σ_s (t : ptr_id) l scs :
     bor_interp σ_t σ_s -∗
-    l ↦t∗[local]{t} scs -∗
+    l ↦t∗[tk_local]{t} scs -∗
     t $$ tk_local -∗
-    ⌜read_mem l (length scs) σ_t.(shp) = Some scs⌝ ∗
-    ⌜∀ i:nat, (i < length scs)%nat → σ_t.(sst) !! (l +ₗ i) = Some [mkItem Unique (Tagged t) None]⌝ ∗
+    ⌜∀ i : nat, (i < length scs)%nat → σ_t.(shp) !! (l +ₗ i) = scs !! i⌝ ∗
+    ⌜∀ i:nat, (i < length scs)%nat → bor_state_own (l +ₗ i) t tk_local σ_t⌝ ∗
     ⌜scs <<t σ_t.(snp)⌝.
   Proof.
-  Admitted.
+    iIntros "(% & % & % & % & (Hc & Htag_auth & Htag_t_auth & Htag_s_auth) & Hsrel & ? & %Htag_interp & %Hwf_s & %Hwf_t)".
+    iIntros "Hp Htag".
+    iPoseProof (tkmap_lookup with "Htag_auth Htag") as "%Htag_lookup".
+    destruct Htag_interp as (Htag_interp & _ & _).
+    destruct (Htag_interp _ _ Htag_lookup) as (_ & _ & Ht & Hs & Hagree).
+    iPoseProof (ghost_map_array_tag_lookup with "Htag_t_auth Hp") as "%Ht_lookup".
+    iPureIntro.
+    enough (∀ i: nat, (i < length scs)%nat → σ_t.(shp) !! (l +ₗ i) = scs !! i ∧ σ_t.(sst) !! (l +ₗ i) = Some [mkItem Unique (Tagged t) None] ∧ wf_scalar σ_t.(snp) (scs !!! i)) as Hsingle.
+    { split_and!; [ apply Hsingle.. | apply tag_values_included_iff; apply Hsingle]. }
+    intros i Hi.
+    specialize (Ht_lookup i Hi). rewrite list_lookup_lookup_total in Ht_lookup; first last.
+    { by apply lookup_lt_is_Some_2. }
+    specialize (Ht _ _ Ht_lookup) as Hcontrol.
+    specialize (loc_controlled_local _ _ _ _ Hcontrol) as (Hstack & Hmem).
+    split_and!.
+    - rewrite Hmem. rewrite list_lookup_lookup_total; [done | by apply lookup_lt_is_Some_2].
+    - done.
+    - intros tg l' Hl.
+      destruct tg as [tg | ]; last done.
+      eapply state_wf_mem_tag; first done.
+      erewrite Hmem, Hl. done.
+  Qed.
 
-  Lemma heap_local_access_source σ_t σ_s (t : ptr_id) l sc :
+  Lemma heap_protected_readN_target σ_t σ_s (t : ptr_id) tk l v_t c M :
+    (∀ i: nat, (i < length v_t)%nat → call_set_in M t (l +ₗ i)) →
     bor_interp σ_t σ_s -∗
-    l ↦s[local]{t} sc -∗
-    t $$ tk_local -∗
-    ⌜σ_s.(shp) !! l = Some sc⌝ ∗
-    ⌜σ_s.(sst) !! l = Some [mkItem Unique (Tagged t) None]⌝ ∗
-    ⌜wf_scalar σ_s sc⌝ ∗
-    (∀ sc',
-      ⌜wf_scalar σ_s sc' ⌝ -∗
-      (*stack_wf st' σ_t -∗ *)
-      |==>
-      bor_interp σ_t (state_upd_mem (<[l := sc']>) σ_s) ∗
-      l ↦s[local]{t} sc').
+    l ↦t∗[tk]{t} v_t -∗
+    t $$ tk -∗
+    c @@ M -∗
+    ⌜∀ i : nat, (i < length v_t)%nat → σ_t.(shp) !! (l +ₗ i) = v_t !! i⌝ ∗
+    ⌜∀ i:nat, (i < length v_t)%nat → bor_state_own (l +ₗ i) t tk σ_t⌝ ∗
+    ⌜v_t <<t σ_t.(snp)⌝.
   Proof.
-  Admitted.
+    iIntros (Hprot) "(% & % & % & % & (Hc & Htag_auth & Htag_t_auth & Htag_s_auth) & Hsrel & %Hcall & %Htag_interp & %Hwf_s & %Hwf_t)".
+    iIntros "Hp Htag Hcall".
+    iPoseProof (tkmap_lookup with "Htag_auth Htag") as "%Htag_lookup".
+    destruct Htag_interp as (Htag_interp & _ & _).
+    destruct (Htag_interp _ _ Htag_lookup) as (_ & _ & Ht & Hs & Hagree).
+    iPoseProof (ghost_map_array_tag_lookup with "Htag_t_auth Hp") as "%Ht_lookup".
+    iPoseProof (ghost_map_lookup with "Hc Hcall") as "%Hc_lookup".
+    iPureIntro.
+    enough (∀ i: nat, (i < length v_t)%nat → σ_t.(shp) !! (l +ₗ i) = v_t !! i ∧ bor_state_own (l +ₗ i) t tk σ_t ∧ wf_scalar σ_t.(snp) (v_t !!! i)) as Hsingle.
+    { split_and!; [ apply Hsingle.. | apply tag_values_included_iff; apply Hsingle]. }
+    intros i Hi.
+    specialize (Ht_lookup i Hi). rewrite list_lookup_lookup_total in Ht_lookup; first last.
+    { by apply lookup_lt_is_Some_2. }
+    specialize (Ht _ _ Ht_lookup) as Hcontrol.
+    assert (bor_state_pre (l +ₗ i) t tk σ_t) as Hpre.
+    { specialize (Hprot i Hi).
+      specialize (call_set_interp_access _ _ _ _ _ Hcall ltac:(exists M; done)). apply loc_protected_bor_state_pre.
+    }
+    specialize (Hcontrol Hpre) as [Hown Hmem].
+    split_and!; [| done | ].
+    - rewrite Hmem. rewrite list_lookup_lookup_total; [done | ]. by apply lookup_lt_is_Some_2.
+    - intros tg l' Hl.
+      destruct tg as [tg | ]; last done.
+      eapply state_wf_mem_tag; first done.
+      erewrite Hmem, Hl. done.
+  Qed.
 
-  Lemma heap_local_accessN_source σ_t σ_s (t : ptr_id) l scs :
-    bor_interp σ_t σ_s -∗
-    l ↦s∗[local]{t} scs -∗
-    t $$ tk_local -∗
-    ⌜read_mem l (length scs) σ_s.(shp) = Some scs⌝ ∗
-    ⌜∀ i:nat, (i < length scs)%nat → σ_s.(sst) !! (l +ₗ i) = Some [mkItem Unique (Tagged t) None]⌝ ∗
-    ⌜scs <<t σ_s.(snp)⌝ ∗
-    (∀ scs',
-      ⌜length scs' = length scs⌝ -∗
-      ⌜scs' <<t σ_s.(snp)⌝ -∗
-      (*stack_wf st' σ_t -∗ *)
-      |==>
-      bor_interp σ_t (state_upd_mem (write_mem l scs') σ_s) ∗
-      l ↦s∗[local]{t} scs').
+  Lemma state_upd_mem_compose f g σ :
+    state_upd_mem f (state_upd_mem g σ) = state_upd_mem (f ∘ g) σ.
+  Proof. destruct σ. done. Qed.
+
+  Lemma write_mem_insert_commute_1 l l' v sc M :
+    l.2 < l'.2 →
+    <[ l := sc ]> (write_mem l' v M) = write_mem l' v (<[ l := sc ]> M).
   Proof.
-  Admitted.
+    induction v in l, l', sc, M |-*; cbn; first done.
+    intros Hl. rewrite (IHv l (l' +ₗ 1)); first last.
+    { destruct l', l; cbn in *; lia. }
+    rewrite insert_commute; first done. intros ->; lia.
+  Qed.
+  Lemma write_mem_head l sc v M :
+    <[ l := sc ]> (write_mem (l +ₗ 1) v M) = write_mem l (sc :: v) M.
+  Proof. rewrite write_mem_insert_commute_1; last by destruct l; cbn; lia. done. Qed.
+
+  Global Instance state_upd_mem_proper : Proper ((eq ==> eq) ==> eq ==> eq) state_upd_mem.
+  Proof.
+    intros f g Heq ? σ ->. destruct σ as [ mem ]. by rewrite /state_upd_mem (Heq mem mem eq_refl).
+  Qed.
+  Lemma state_upd_write_mem_head sc v l σ :
+    state_upd_mem (<[ l := sc ]> ∘ write_mem (l +ₗ 1) v) σ = state_upd_mem (write_mem l (sc :: v)) σ.
+  Proof. destruct σ. rewrite /state_upd_mem. cbn. by rewrite write_mem_head. Qed.
+
+  Lemma heap_local_writeN_target σ_t σ_s (t : ptr_id) l scs scs' :
+    bor_interp σ_t σ_s -∗
+    l ↦t∗[tk_local]{t} scs -∗
+    t $$ tk_local -∗
+    ⌜length scs' = length scs⌝ -∗
+    ⌜scs' <<t σ_t.(snp) ⌝ ==∗
+    bor_interp (state_upd_mem (write_mem l scs') σ_t) σ_s ∗
+    l ↦t∗[tk_local]{t} scs' ∗
+    t $$ tk_local.
+  Proof.
+    iInduction scs' as [ | sc' scs'] "IH" forall (l scs).
+    - iIntros "Hbor Hp Ht %Hlen _". destruct scs; last done. iFrame "Ht Hp". iModIntro. destruct σ_t; eauto.
+    - iIntros "Hbor Hp Ht %Hlen %Hwf". destruct scs as [ | sc scs]; first done.
+      iPoseProof (big_sepL_cons with "Hp") as "[Hh Hp]".
+      iMod  ("IH" $! (l +ₗ 1) scs with "Hbor [Hp] Ht [] []") as "(Hbor & Hp & Ht)".
+      { iApply (big_sepL_mono with "Hp"). intros i sc0 Hsc0. cbn.
+        rewrite shift_loc_assoc. replace (1 + i)%Z with (Z.of_nat $ S i) by lia. done. }
+      { cbn in Hlen. iPureIntro. lia. }
+      { iPureIntro. intros l' tg Hin. eapply Hwf. right. apply Hin. }
+      iMod (heap_local_write_target  _ _ _ _ _ sc' with "Hbor Hh Ht []") as "(Hbor & Hh & Ht)".
+      { iPureIntro. cbn. specialize (proj1 (tag_values_included_iff _ _) Hwf) as Hi. apply (Hi O). cbn; lia. }
+      iModIntro. iFrame "Ht". iSplitL "Hbor".
+      { rewrite state_upd_mem_compose. rewrite shift_loc_0_nat. by rewrite state_upd_write_mem_head. }
+      iApply big_sepL_cons. iFrame "Hh". iApply (big_sepL_mono with "Hp").
+      intros i sc0 Hsc0. cbn.
+      rewrite shift_loc_assoc. replace (1 + i)%Z with (Z.of_nat $ S i) by lia. done.
+  Qed.
 
   Lemma heap_local_readN_source σ_t σ_s (t : ptr_id) l scs :
     bor_interp σ_t σ_s -∗
-    l ↦s∗[local]{t} scs -∗
+    l ↦s∗[tk_local]{t} scs -∗
     t $$ tk_local -∗
-    ⌜read_mem l (length scs) σ_s.(shp) = Some scs⌝ ∗
-    ⌜∀ i:nat, (i < length scs)%nat → σ_s.(sst) !! (l +ₗ i) = Some [mkItem Unique (Tagged t) None]⌝ ∗
+    ⌜∀ i : nat, (i < length scs)%nat → σ_s.(shp) !! (l +ₗ i) = scs !! i⌝ ∗
+    ⌜∀ i:nat, (i < length scs)%nat → bor_state_own (l +ₗ i) t tk_local σ_s⌝ ∗
     ⌜scs <<t σ_s.(snp)⌝.
+  Proof.
+  Admitted.
+
+  Lemma heap_local_writeN_source σ_t σ_s (t : ptr_id) l scs scs' :
+    bor_interp σ_t σ_s -∗
+    l ↦s∗[tk_local]{t} scs -∗
+    t $$ tk_local -∗
+    ⌜length scs' = length scs⌝ -∗
+    ⌜scs' <<t σ_s.(snp) ⌝ ==∗
+    bor_interp σ_t (state_upd_mem (write_mem l scs') σ_s) ∗
+    l ↦s∗[tk_local]{t} scs' ∗
+    t $$ tk_local.
   Proof.
   Admitted.
 
@@ -840,6 +1008,7 @@ Lemma local_access_eq l t t' stk n stk' kind σ_s σ_t M_tag M_t M_s :
 Proof.
   intros Hst Haccess Htag Ht Htag_interp.
   specialize (access1_in_stack _ _ _ _ _ _ Haccess) as (it & Hin_stack & <- & Henabled).
+  destruct Htag_interp as (Htag_interp & _ & _).
   specialize (Htag_interp _ _ Htag) as (_ & _ & Htl & Hsl & Hdom).
   destruct Ht as (sc_t & Ht).
   specialize (Htl _ _ Ht) as Hcontrol.
@@ -849,7 +1018,6 @@ Proof.
   rewrite Hcontrol => [= <-]. rewrite elem_of_list_singleton => ->.
   rewrite Hn => [= _ <-]. done.
 Qed.
-
 
 Lemma protector_access_eq l t t' stk n stk' kind σ_s σ_t M_tag Mcall M_t M_s :
   σ_t.(sst) !! l = Some stk →
@@ -864,6 +1032,7 @@ Lemma protector_access_eq l t t' stk n stk' kind σ_s σ_t M_tag Mcall M_t M_s :
 Proof.
   intros Hst Haccess Htag Ht (c & Hcall) Htag_interp Hcall_interp Hwf.
   specialize (call_set_interp_access _ _ _ _ _ Hcall_interp Hcall) as (Hc_in & _ & (stk'' & pm & Hstk'' & Hin & Hpm)).
+  destruct Htag_interp as (Htag_interp & _ & _).
   specialize (Htag_interp _ _ Htag) as (_ & _ & Htl & Hsl & Hdom).
   destruct Ht as (sc_t & Ht).
   specialize (Htl _ _ Ht) as Hcontrol.
@@ -890,7 +1059,7 @@ Proof.
   intros Hs ([? ?] & Haccess) Hpriv Htag_interp Hcall_interp Hwf.
   destruct Hpriv as (tk & Htag & Ht & [-> | [-> Hc]]).
   - by eapply local_access_eq.
-  - by eapply protector_access_eq.
+  - eapply protector_access_eq; done.
 Qed.
 
 Definition untagged_or_public (M_tag : gmap ptr_id (tag_kind * unit)) t :=
@@ -913,6 +1082,27 @@ Proof.
   destruct Hpriv as (tk & Hl & _ & [-> | [-> _]]); cbn; intros; simplify_eq.
 Qed.
 
+Lemma priv_loc_UB_retag_access_eq σ_s σ_t c l old new mut T kind α' nxtp' M_tag M_t M_s Mcall
+  (FRZ: if mut is Immutable then is_freeze T else True)
+  (N2P: kind ≠ TwoPhase) :
+  retag σ_t.(sst) σ_t.(snp) σ_t.(scs) c l old kind (RefPtr mut) T = Some (new, α', nxtp') →
+  ∀ i t, (i < tsize T)%nat →
+  priv_loc M_tag M_t Mcall t (l +ₗ i) →
+  tag_interp M_tag M_t M_s σ_t σ_s →
+  call_set_interp Mcall σ_t →
+  state_wf σ_t →
+  untagged_or_public M_tag old →
+  False.
+Proof.
+  intros Hrt i t Hi.
+  have NZST: (0 < tsize T)%nat by lia.
+  destruct (retag_change_ref_NZST _ _ _ _ _ _ _ _ _ _ _ _ NZST Hrt);
+    subst new nxtp'.
+  destruct (retag_Some_Ref _ _ _ _ _ _ _ _ _ _ _ _ NZST FRZ N2P Hrt _ Hi)
+    as (stk & stk' & Eqstk & Eqstk' & GR).
+  apply grant_access1 in GR; [|by destruct mut].
+  revert Eqstk GR. by apply priv_pub_access_UB.
+Qed.
 
 
 (* NOTE: might need to generalize that with the bijection a bit when we want to do cool things, e.g., pass parts of an object to a function (but for just obtaining a reflexivity thm, it should be fine) *)
@@ -988,34 +1178,34 @@ Section val_rel.
   Proof. iIntros "Hrel"; destruct sc_t; [done.. | ]. by iDestruct "Hrel" as "->". Qed.
 
   Lemma rrel_place_source r_t l_s t_s T :
-    rrel r_t (PlaceR l_s t_s T) -∗ 
+    rrel r_t (PlaceR l_s t_s T) -∗
     ∃ l_t, ⌜r_t = PlaceR l_t t_s T⌝ ∗ (if t_s is Tagged t then t $$ tk_pub else True).
   Proof.
     iIntros "Hrel".
     destruct r_t as [ | l_t t' T']; first done. iDestruct "Hrel" as "(#H & ->)".
-    iDestruct (sc_rel_ptr_source with "H") as "[%Heq Htag]". 
+    iDestruct (sc_rel_ptr_source with "H") as "[%Heq Htag]".
     injection Heq as [= -> ->]. iExists l_s. eauto.
   Qed.
-  Lemma rrel_value_source r_t v_s : 
-    rrel r_t (ValR v_s) -∗ 
-    ∃ v_t, ⌜r_t = ValR v_t⌝ ∗ value_rel v_t v_s. 
-  Proof. 
+  Lemma rrel_value_source r_t v_s :
+    rrel r_t (ValR v_s) -∗
+    ∃ v_t, ⌜r_t = ValR v_t⌝ ∗ value_rel v_t v_s.
+  Proof.
     iIntros "Hrel". destruct r_t as [ v_t | ]; last done.
     iExists v_t. iFrame "Hrel". done.
   Qed.
 
 
-  Lemma value_rel_length v_t v_s : 
+  Lemma value_rel_length v_t v_s :
     value_rel v_t v_s -∗ ⌜length v_t = length v_s⌝.
   Proof. iApply big_sepL2_length. Qed.
-  Lemma value_rel_empty : 
+  Lemma value_rel_empty :
     ⊢ value_rel [] [].
   Proof. by iApply big_sepL2_nil. Qed.
 
-  Lemma value_rel_singleton_source v_t sc_s : 
+  Lemma value_rel_singleton_source v_t sc_s :
     value_rel v_t [sc_s] -∗ ∃ sc_t, ⌜v_t = [sc_t]⌝ ∗ sc_rel sc_t sc_s.
-  Proof. 
-    iIntros "Hv". iPoseProof (value_rel_length with "Hv") as "%Hlen". 
+  Proof.
+    iIntros "Hv". iPoseProof (value_rel_length with "Hv") as "%Hlen".
     destruct v_t as [ | sc_t []]; [done | | done ].
     iExists sc_t. iSplitR "Hv"; first done. iRevert "Hv". rewrite /value_rel big_sepL2_singleton. eauto.
   Qed.
@@ -1056,8 +1246,8 @@ Proof. rewrite /fresh_block. intros ->. done. Qed.
 (* reflexivity steps *)
 Lemma sim_alloc_local T Φ π :
   (∀ t l_t l_s, t $$ tk_local -∗
-    l_t ↦t∗[local]{t} repeat ScPoison (tsize T) -∗
-    l_s ↦s∗[local]{t} repeat ScPoison (tsize T) -∗
+    l_t ↦t∗[tk_local]{t} repeat ScPoison (tsize T) -∗
+    l_s ↦s∗[tk_local]{t} repeat ScPoison (tsize T) -∗
     Place l_t (Tagged t) T ⪯{π, Ω} Place l_s (Tagged t) T [{ Φ }]) -∗
   Alloc T ⪯{π, Ω} Alloc T [{ Φ }].
 Proof.
@@ -1073,7 +1263,7 @@ Proof.
   iModIntro.
   iExists (Place l_s (Tagged (σ_t.(snp))) T), [], (mkState (init_mem l_s (tsize T) σ_s.(shp)) (init_stacks σ_s.(sst) l_s (tsize T) (Tagged σ_s.(snp))) σ_s.(scs) (S σ_s.(snp)) σ_s.(snc)).
   iFrame. iSplitR.
-  { iPureIntro. destruct Hp as (<- & _).  econstructor 2; econstructor. }
+  { iPureIntro. destruct Hp as (_ & <- & _).  econstructor 2; econstructor. }
   iSplitL; last by iApply big_sepL2_nil.
   iApply ("Hsim" with "Htag Htarget Hsource").
 Qed.
@@ -1086,11 +1276,34 @@ Lemma sim_alloc_public T Φ π :
 Proof.
 Admitted.
 
-(* TODO: local ownership makes strong assertions: 
+(* TODO: local ownership makes strong assertions:
   we also have to deallocate the corresponding ghost state *)
 (*Lemma sim_free_local : *)
 
   (*Free (Place l t T_t) ⪯{π, Ω*)
+
+Lemma bor_state_own_access1_read l t tk stk σ :
+  bor_state_own l t tk σ →
+  σ.(sst) !! l = Some stk →
+  ∃ n, access1 stk AccessRead (Tagged t) σ.(scs) = Some (n, stk).
+Proof.
+  intros Hown. destruct tk; cbn in *.
+  - destruct Hown as (st & -> & Hsro). move => [= <-]. by apply tag_SRO_top_access.
+  - destruct Hown as (st & Hsst & (opro & st' & H)). simplify_eq. rewrite Hsst => [= <-].
+    eapply tag_unique_head_access. eexists; eauto.
+  - rewrite Hown => [= <-].
+    eapply tag_unique_head_access. eexists; eauto.
+Qed.
+
+Lemma memory_read_access1 (stks : stacks) l n t calls :
+  (∀ i: nat, (i < n)%nat → ∃ stk, stks !! (l +ₗ i) = Some stk ∧ ∃ m, access1 stk AccessRead (Tagged t) calls = Some (m, stk)) →
+  memory_read stks calls l (Tagged t) n = Some stks.
+Proof.
+  induction n as [ | n IH]; cbn; first done.
+  intros Hacc1. destruct (Hacc1 n ltac:(lia)) as (stkn & Hl & (m & Hacc1_n)). rewrite Hl.
+  cbn. rewrite Hacc1_n. cbn.
+  rewrite insert_id; last done. apply IH. intros i Hi. apply Hacc1. lia.
+Qed.
 
 Lemma sim_free_public T_t T_s l_t l_s bor_t bor_s Φ π :
   rrel (PlaceR l_t bor_t T_t) (PlaceR l_s bor_s T_s) -∗
@@ -1166,7 +1379,6 @@ Proof.
     done.
 Qed.
 
-
 Lemma sim_copy_public Φ π l_t bor_t T_t l_s bor_s T_s :
   rrel (PlaceR l_t bor_t T_t) (PlaceR l_s bor_s T_s) -∗
   (∀ v_t v_s, value_rel v_t v_s -∗ v_t ⪯{π, Ω} ValR v_s [{ Φ }]) -∗
@@ -1241,18 +1453,18 @@ Proof.
       specialize (for_each_access1_active_preserving _ _ _ _ _ _ _ ACC l stk Hstk_some) as (stk' & Hstk'_some & Hac_pres).
       exists stk', pm. split; last split; [ done | by apply Hac_pres| done ].
     - (* tag invariant *)
-      iPureIntro.
+      iPureIntro. destruct Htag_interp as (Htag_interp & Ht_dom & Hs_dom). split_and!; [ | done..].
       intros t tk Htk_some. destruct (Htag_interp t tk Htk_some) as (Hsnp_lt_t & Hsnp_lt_s & Hctrl_t & Hctrl_s & Hag).
       split_and!; [ done | done | | | done ].
       + intros l sc_t Hsc_t. eapply sim_copy_public_controlled_update; [ by eauto .. | | by eauto].
         intros stk n t' stk' kind Hstk Hacc1 ->.
-        eapply (local_access_eq _ _ _ _ _ _ _ _ _ _ _ _ Hstk Hacc1 Htk_some ltac:(eauto) Htag_interp).
+        eapply (local_access_eq _ _ _ _ _ _ _ _ _ _ _ _ Hstk Hacc1 Htk_some ltac:(eauto) ltac:(done)).
       + intros l sc_s Hsc_s. eapply sim_copy_public_controlled_update; [ by eauto .. | | by eauto].
         intros stk n t' stk' kind Hstk Hacc1 ->.
         rewrite Hstacks_eq in Hstk. rewrite Hcalls_eq in Hacc1.
         assert (is_Some (M_t !! (t, l))) as Ht_some.
         { apply Hag. eauto. }
-        eapply (local_access_eq _ _ _ _ _ _ _ _ _ _ _ _ Hstk Hacc1 Htk_some Ht_some Htag_interp).
+        eapply (local_access_eq _ _ _ _ _ _ _ _ _ _ _ _ Hstk Hacc1 Htk_some Ht_some ltac:(done)).
     - (* source state wf *)
       iPureIntro. eapply head_step_wf; done.
     - (* target state wf *)
@@ -1264,8 +1476,9 @@ Proof.
   (* proving the value relation *)
   specialize (read_mem_values _ _ _ _ COPY) as [Hlen_t Hv_t].
   specialize (read_mem_values _ _ _ _ Hread_s) as [Hlen_s Hv_s].
-  iApply big_sepL2_intuitionistically_forall; first lia.
-  iModIntro. iIntros (i sc_t sc_s) "%Hs_t %Hs_v".
+
+  iApply big_sepL2_forall; iSplit; first (iPureIntro;lia).
+  iIntros (i sc_t sc_s) "%Hs_t %Hs_v".
   assert (i < tsize T_t)%nat as Hi. { rewrite -Hlen_t. eapply lookup_lt_is_Some_1. eauto. }
   iPoseProof (state_rel_pub_if_not_priv _ _ _ _ _ _ (l_t +ₗ i) with "[] Hsrel [Hrel]") as "Hpub".
   { iPureIntro. by apply Hsome_target. }
@@ -1287,8 +1500,8 @@ Qed.
 Lemma target_copy_local v_t T l t Ψ :
   length v_t = tsize T →
   t $$ tk_local -∗
-  l ↦t∗[local]{t} v_t -∗
-  (l ↦t∗[local]{t} v_t -∗ t $$ tk_local -∗ target_red #v_t Ψ)%E -∗
+  l ↦t∗[tk_local]{t} v_t -∗
+  (l ↦t∗[tk_local]{t} v_t -∗ t $$ tk_local -∗ target_red #v_t Ψ)%E -∗
   target_red (Copy (Place l (Tagged t) T)) Ψ.
 Proof.
   iIntros (Hlen) "Htag Ht Hsim".
@@ -1296,48 +1509,28 @@ Proof.
   iModIntro.
   iPoseProof (heap_local_readN_target with "Hbor Ht Htag") as "(%Hd & %Hstack & %Hwf)".
   rewrite Hlen in Hd Hstack.
+  have READ_t : read_mem l (tsize T) σ_t.(shp) = Some v_t.
+  { apply read_mem_values'; done. }
   iPoseProof (bor_interp_get_state_wf with "Hbor") as "[%Hwf_t %]".
+  have Eq_stk : memory_read σ_t.(sst) σ_t.(scs) l (Tagged t) (tsize T) = Some σ_t.(sst).
+  { apply memory_read_access1. intros i Hi.
+    specialize (Hstack i Hi). eexists; split; first done. eapply bor_state_own_access1_read; done. }
   iSplitR.
-  { iPureIntro.
-    edestruct (copy_head_step P_t σ_t l (Tagged t) T) as (v & α & Hread & Hnewstack & Hhead);
-      last (do 3 eexists; eapply Hhead).
-    - done.
-    - apply read_mem_is_Some'. eauto.
-    - intros m stk Hm Hst. rewrite /access1_read_pre.
-      rewrite Hstack in Hst; last lia. injection Hst as [= <-].
-      exists 0%nat, (mkItem Unique (Tagged t) None).
-      split_and!; [done.. |]. intros ? ? ?; lia.
-  }
+  { iPureIntro. do 3 eexists; eapply copy_head_step'; [done | done | eauto ]. }
   iIntros (e_t' efs_t σ_t') "%Hhead".
   specialize (head_copy_inv _ _ _ _ _ _ _ _ Hhead) as (v_t' & α' & -> & READ & ACC & BOR & -> & ->).
-  rewrite READ in Hd. simplify_eq.
+  rewrite READ in READ_t. simplify_eq.
   iModIntro. iSplitR; first done.
   iFrame "HP_t HP_s".
   iSplitL "Hbor"; last iApply ("Hsim" with "Ht Htag").
-
-  assert (α' = σ_t.(sst)) as ->.
-  {
-    apply map_eq. intros l'.
-    specialize (for_each_dom _ _ _ _ _ ACC) as Hdom.
-    destruct ((sst σ_t) !! l') as [stk | ] eqn:Hst; first last.
-    { rewrite Hst. apply not_elem_of_dom in Hst. move : Hst. rewrite Hdom. apply not_elem_of_dom. }
-    specialize (proj2 (elem_of_dom σ_t.(sst) l') ltac:(eauto)) as Hel. move: Hel.
-    rewrite Hdom. intros (stk' & Hst')%elem_of_dom.
-    specialize (for_each_lookup_case _ _ _ _ _ ACC l' stk stk' Hst Hst') as [Heq | [Hacc1 (i & Hi & ->)]].
-    { by rewrite Hst Hst' Heq. }
-    specialize (Hstack i ltac:(lia)).
-    rewrite Hst in Hstack. injection Hstack as [=].
-    specialize (tag_unique_head_access σ_t.(scs) stk (Tagged t) None AccessRead ltac:(exists []; eauto)) as (n & Hacc_eq).
-    rewrite Hacc_eq in Hacc1. injection Hacc1 as [= <-]. by rewrite Hst Hst'.
-  }
   destruct σ_t; done.
 Qed.
 
 Lemma source_copy_local v_s T l t Ψ π :
   length v_s = tsize T →
   t $$ tk_local -∗
-  l ↦s∗[local]{t} v_s -∗
-  (l ↦s∗[local]{t} v_s -∗ t $$ tk_local -∗ source_red #v_s π Ψ)%E -∗
+  l ↦s∗[tk_local]{t} v_s -∗
+  (l ↦s∗[tk_local]{t} v_s -∗ t $$ tk_local -∗ source_red #v_s π Ψ)%E -∗
   source_red (Copy (Place l (Tagged t) T)) π Ψ.
 Proof.
   iIntros (Hlen) "Htag Hs Hsim".
@@ -1346,36 +1539,18 @@ Proof.
   iPoseProof (bor_interp_get_state_wf with "Hbor") as "[% %Hwf_s]".
   iPoseProof (heap_local_readN_source with "Hbor Hs Htag") as "(%Hd & %Hstack & %Hwf)".
   rewrite Hlen in Hd Hstack.
+  have READ_s : read_mem l (tsize T) σ_s.(shp) = Some v_s.
+  { apply read_mem_values'; done. }
+  have Eq_stk : memory_read σ_s.(sst) σ_s.(scs) l (Tagged t) (tsize T) = Some σ_s.(sst).
+  { apply memory_read_access1. intros i Hi.
+    specialize (Hstack i Hi). eexists; split; first done. eapply bor_state_own_access1_read; done. }
   assert (head_reducible P_s (Copy (Place l (Tagged t) T)) σ_s) as (e_s' & σ_s' & efs & Hhead).
-  { edestruct (copy_head_step P_s σ_s l (Tagged t) T) as (v & α & Hread & Hnewstack & Hhead);
-      last (do 3 eexists; eapply Hhead).
-    - done.
-    - apply read_mem_is_Some'. eauto.
-    - intros m stk Hm Hst. rewrite /access1_read_pre.
-      rewrite Hstack in Hst; last lia. injection Hst as [= <-].
-      exists 0%nat, (mkItem Unique (Tagged t) None).
-      split_and!; [done.. |]. intros ? ? ?; lia.
-  }
+  { do 3 eexists; eapply copy_head_step'; [done | done | eauto ]. }
   iExists e_s', σ_s'.
   specialize (head_copy_inv _ _ _ _ _ _ _ _ Hhead) as (v_t' & α' & -> & READ & ACC & BOR & -> & ->).
-  rewrite READ in Hd. simplify_eq.
+  rewrite READ in READ_s. simplify_eq.
   iFrame "HP_t HP_s". iSplitR; first done.
   iSplitL "Hbor"; last by iApply ("Hsim" with "Hs Htag"). iModIntro.
-  assert (α' = σ_s.(sst)) as ->.
-  {
-    apply map_eq. intros l'.
-    specialize (for_each_dom _ _ _ _ _ ACC) as Hdom.
-    destruct ((sst σ_s) !! l') as [stk | ] eqn:Hst; first last.
-    { rewrite Hst. apply not_elem_of_dom in Hst. move : Hst. rewrite Hdom. apply not_elem_of_dom. }
-    specialize (proj2 (elem_of_dom σ_s.(sst) l') ltac:(eauto)) as Hel. move: Hel.
-    rewrite Hdom. intros (stk' & Hst')%elem_of_dom.
-    specialize (for_each_lookup_case _ _ _ _ _ ACC l' stk stk' Hst Hst') as [Heq | [Hacc1 (i & Hi & ->)]].
-    { by rewrite Hst Hst' Heq. }
-    specialize (Hstack i ltac:(lia)).
-    rewrite Hst in Hstack. injection Hstack as [=].
-    specialize (tag_unique_head_access σ_s.(scs) stk (Tagged t) None AccessRead ltac:(exists []; eauto)) as (n & Hacc_eq).
-    rewrite Hacc_eq in Hacc1. injection Hacc1 as [= <-]. by rewrite Hst Hst'.
-  }
   by destruct σ_s.
 Qed.
 
@@ -1389,7 +1564,31 @@ Lemma target_copy_protected v_t T l t tk Ψ c M  :
   (l ↦t∗[tk]{t} v_t -∗ c @@ M -∗ t $$ tk -∗ target_red #v_t Ψ)%E -∗
   target_red (Copy (Place l (Tagged t) T)) Ψ.
 Proof.
-Admitted.
+  iIntros (Hlen Hprotected) "Hcall Htag Ht Hsim".
+  iApply target_red_lift_head_step. iIntros (?????) "(HP_t & HP_s & Hbor)".
+  iModIntro.
+  iPoseProof (heap_protected_readN_target with "Hbor Ht Htag Hcall") as "(%Hd & %Hown & %Hwf)".
+  { by rewrite Hlen. }
+  rewrite Hlen in Hd Hown.
+  have READ_t : read_mem l (tsize T) σ_t.(shp) = Some v_t.
+  { apply read_mem_values'; done. }
+  iPoseProof (bor_interp_get_state_wf with "Hbor") as "[%Hwf_t %]".
+  have Eq_stk : memory_read σ_t.(sst) σ_t.(scs) l (Tagged t) (tsize T) = Some σ_t.(sst).
+  {
+    apply memory_read_access1. intros i Hi.
+    specialize (Hown i Hi). destruct (bor_state_own_some_stack _ _ _ _ Hown) as (stk & Hs_stk).
+    exists stk. split; first done. eapply bor_state_own_access1_read; done.
+  }
+  iSplitR.
+  { iPureIntro. do 3 eexists; eapply copy_head_step'; [done | eapply read_mem_values'; eauto | eauto]. }
+  iIntros (e_t' efs_t σ_t') "%Hhead".
+  specialize (head_copy_inv _ _ _ _ _ _ _ _ Hhead) as (v_t' & α' & -> & READ & ACC & BOR & -> & ->).
+  rewrite READ in READ_t. simplify_eq.
+  iModIntro. iSplitR; first done.
+  iFrame "HP_t HP_s".
+  iSplitL "Hbor"; last iApply ("Hsim" with "Ht Hcall Htag").
+  destruct σ_t; done.
+Qed.
 
 (* doesn't need protectors due to source UB *)
 Lemma source_copy_any v_s T l t tk Ψ π :
@@ -1415,9 +1614,9 @@ Admitted.
 *)
 Lemma sim_write_unique_unprotected π l_t l_s t T v_t v_s v_t' v_s' Φ :
   t $$ tk_unq -∗
-  l_t ↦t∗[unq]{t} v_t -∗
-  l_s ↦s∗[unq]{t} v_s -∗
-  (t $$ tk_unq -∗ l_t ↦t∗[unq]{t} v_t' -∗ l_s ↦s∗[unq]{t} v_s' -∗ #[☠] ⪯{π, Ω} #[☠] [{ Φ }]) -∗
+  l_t ↦t∗[tk_unq]{t} v_t -∗
+  l_s ↦s∗[tk_unq]{t} v_s -∗
+  (t $$ tk_unq -∗ l_t ↦t∗[tk_unq]{t} v_t' -∗ l_s ↦s∗[tk_unq]{t} v_s' -∗ #[☠] ⪯{π, Ω} #[☠] [{ Φ }]) -∗
   Write (Place l_t (Tagged t) T) #v_t' ⪯{π, Ω} Write (Place l_s (Tagged t) T) #v_s' [{ Φ }].
 Proof.
 Admitted.
@@ -1473,17 +1672,317 @@ Lemma sim_retag_public l_t l_s ot os c kind T rkind π Φ :
 Proof.
 Admitted.
 
+Lemma head_retag_inv (P : prog) σ σ' e' efs l ot c pkind T rkind :
+  head_step P (Retag #[ScPtr l ot] #[ScCallId c] pkind T rkind) σ e' σ' efs →
+  ∃ nt α' nxtp',
+  retag σ.(sst) σ.(snp) σ.(scs) c l ot rkind pkind T = Some (nt, α', nxtp') ∧
+  e' = (#[ScPtr l nt])%E ∧
+  efs = [] ∧
+  σ' = mkState σ.(shp) α' σ.(scs) nxtp' σ.(snc) ∧
+  c ∈ σ.(scs).
+Proof. intros Hhead. inv_head_step. eauto 8. Qed.
+
+Lemma lookup_union_Some_l' `{EqDecision K} `{Countable K} V (M1 M2 : gmap K V) (k : K) (v : V) :
+  (M1 ∪ M2) !! k = Some v → M2 !! k = None → M1 !! k = Some v.
+Proof.
+  destruct (M1 !! k) as [ v' | ] eqn:Hv'.
+  - specialize (lookup_union_Some_l M1 M2 _ _ Hv') as ->. move => [= ->]. done.
+  - rewrite lookup_union_r; last done. congruence.
+Qed.
+Lemma lookup_union_is_Some `{EqDecision K} `{Countable K} V (M1 M2 : gmap K V) (k : K) :
+  is_Some ((M1 ∪ M2) !! k) ↔ is_Some (M1 !! k) ∨ is_Some (M2 !! k). 
+Proof. 
+  split.
+  - intros (v & Hv). destruct (M1 !! k) eqn:HM1; first by eauto.
+    right. erewrite <-lookup_union_r; eauto.
+  - intros [(v & HM1) | (v & HM2)].
+    + rewrite (lookup_union_Some_l _ _ _ _ HM1); eauto.
+    + destruct (M1 !! k) eqn:HM1. { rewrite (lookup_union_Some_l _ _ _ _ HM1); eauto. }
+      rewrite lookup_union_r; eauto. 
+Qed.
+
+Lemma dom_agree_on_tag_union M1_t M1_s M2_t M2_s t : 
+  dom_agree_on_tag M1_t M1_s t → dom_agree_on_tag M2_t M2_s t →
+  dom_agree_on_tag (M1_t ∪ M2_t) (M1_s ∪ M2_s) t.
+Proof.
+  intros [H1a H1b] [H2a H2b]. split; intros l; rewrite !lookup_union_is_Some; naive_solver. 
+Qed.
+
+Lemma dom_agree_on_tag_array_tag_map l t v_t v_s : 
+  length v_t = length v_s →
+  dom_agree_on_tag (array_tag_map l t v_t) (array_tag_map l t v_s) t.
+Proof. 
+  intros Hlen. split; intros l'. 
+  - intros (_ & (i & Hi & ->))%array_tag_map_lookup2. rewrite array_tag_map_lookup_Some; last lia. 
+    apply lookup_lt_is_Some_2. lia. 
+  - intros (_ & (i & Hi & ->))%array_tag_map_lookup2. rewrite array_tag_map_lookup_Some; last lia. 
+    apply lookup_lt_is_Some_2. lia. 
+Qed.
+
+Lemma array_tag_map_lookup_None t t' l v : 
+  t ≠ t' → ∀ l', array_tag_map l t v !! (t', l') = None. 
+Proof. 
+  intros Hneq l'. destruct (array_tag_map l t v !! (t', l')) eqn:Harr; last done.
+  specialize (array_tag_map_lookup1 l t v t' l' ltac:(eauto)) as [Heq _]; congruence. 
+Qed.
+
+Lemma dom_agree_on_tag_not_elem M_t M_s t : 
+  (∀ l, M_t !! (t, l) = None) → (∀ l, M_s !! (t, l) = None) →
+  dom_agree_on_tag M_t M_s t. 
+Proof. intros Ht Hs. split; intros l; rewrite Ht Hs; congruence. Qed.
+
+Lemma retag_default_loc_controlled σ c l ot T mut α' i sc : 
+  let nt := σ.(snp) in
+  let pk := RefPtr mut in 
+  let tk := match mut with Mutable => tk_unq | Immutable => tk_pub end in
+  (if mut is Immutable then is_freeze T else True) →
+  retag σ.(sst) σ.(snp) σ.(scs) c l ot Default pk T = Some (Tagged nt, α', S σ.(snp)) → 
+  (i < tsize T)%nat →
+  σ.(shp) !! (l +ₗ i) = Some sc → 
+  loc_controlled (l +ₗ i) nt tk sc (mkState σ.(shp) α' σ.(scs) (S σ.(snp)) σ.(snc)).
+Proof.
+  intros nt pk tk Hfreeze  Hretag Hi Hsc Hpre. split; last done.
+  destruct mut. 
+  * (* unique *)
+    destruct Hpre as (st & pm' & opro & Hst & Hit & Hpm'). exists st. split; first done.
+    have EqRT':
+      retag_ref σ.(sst) σ.(scs) σ.(snp) l ot T (UniqueRef false) None =
+        Some (Tagged nt, α', S nt) by done.
+    destruct (tag_on_top_retag_ref_uniq _ _ _ _ _ _ _ _ _ _ EqRT' i ltac:(lia))
+      as [pro1 Eqstk1]. rewrite Hst /= in Eqstk1.
+    clear -Eqstk1. destruct st as [|? stk1]; [done|].
+    simpl in Eqstk1. simplify_eq. by exists pro1, stk1.
+  * (* shared *)
+    destruct Hpre as (stk' & pm' & pro & Eqstk' & In' & NDIS). simpl in Eqstk'.
+    exists stk'. split; [done|].
+    have EqRT':
+      retag_ref σ.(sst) σ.(scs) σ.(snp) l ot T SharedRef None = Some (Tagged nt, α', S nt) by done.
+    have HTOP := (tag_on_top_retag_ref_shr _ _ _ _ _ _ _ _ _ _ Hfreeze EqRT' i ltac:(lia)).
+    clear -HTOP Eqstk'.
+    apply tag_on_top_shr_active_SRO in HTOP as (?&?&?). by simplify_eq.
+Qed.
+
+Lemma retag_default_loc_controlled' σ c l l' t tk' ot T mut α' sc :
+  let nt := σ.(snp) in
+  let pk := RefPtr mut in 
+  (if mut is Immutable then is_freeze T else True) →
+  state_wf σ →
+  retag σ.(sst) σ.(snp) σ.(scs) c l ot Default pk T = Some (Tagged nt, α', S σ.(snp)) →
+  (Tagged t = ot → tk' = tk_pub) →
+  nt ≠ t →
+  (t < σ.(snp))%nat →
+  loc_controlled l' t tk' sc σ →
+  loc_controlled l' t tk' sc (mkState σ.(shp) α' σ.(scs) (S σ.(snp)) σ.(snc)).
+Proof. 
+  intros nt pk Hfreeze Hwf Hretag Hneq' Hneq Hlt Hcontrolled. 
+  intros Hpre. destruct tk'. 
+  * destruct Hpre as (stk' & pm' & pro & Eqstk' & In' & ND).
+    destruct (retag_item_in _ _ _ _ _ _ _ _ _ _ _ _ Hretag _ _ t _ Eqstk' In')
+      as (stk & Eqstk & In); [done..|].
+       
+    destruct Hcontrolled as (Hown & Hl'). { simpl; naive_solver. }
+    cbn. split; last done.
+    exists stk'. split; [done|].
+    destruct Hown as (stk1 & Eqstk1 & HTOP).
+    rewrite Eqstk1 in Eqstk. simplify_eq.
+    move : HTOP.
+    have ND2 := proj2 (state_wf_stack_item _ Hwf _ _ Eqstk1).
+    by apply (retag_item_active_SRO_preserving _ _ _ _ _ _ _ _ _ _ _ _ Hretag _ _ _ _ _ ND2 Eqstk1 Eqstk' In In').
+  * destruct Hpre as (stk' & pm' & pro & Eqstk' & In' & ND).
+    destruct (retag_item_in _ _ _ _ _ _ _ _ _ _ _ _ Hretag _ _ t _ Eqstk' In')
+      as (stk & Eqstk & In); [done..|].
+    destruct Hcontrolled as (Hown & Hl'); [simpl; naive_solver|].
+    split; last done. cbn. 
+    exists stk'. split; [done|].
+    destruct Hown as (stk1 & Eqstk1 & opro1 & HTOP).
+    rewrite Eqstk1 in Eqstk. simplify_eq.
+    have ND2 := proj2 (state_wf_stack_item _ Hwf _ _ Eqstk1).
+    assert (opro1 = pro ∧ pm' = Unique) as [].
+    { have In1 : mkItem Unique (Tagged t) opro1 ∈ stk.
+      { destruct HTOP as [? HTOP]. rewrite HTOP. by left. }
+      have EQ := stack_item_tagged_NoDup_eq _ _ _ t ND2 In1 In eq_refl eq_refl.
+      by simplify_eq. } subst opro1 pm'. exists pro.
+    have NEq: Tagged t ≠ ot.
+    { intros <-. specialize (Hneq' eq_refl). congruence. } 
+    move : HTOP.
+    by apply (retag_item_head_preserving _ _ _ _ _ _ _ _ _ _ _ _ Hretag
+                _ _ _ _ _ ND2 Eqstk1 Eqstk' NEq In').
+  * clear Hpre. specialize (Hcontrolled I) as (Hown & Hl'). split; last done.
+    move : Hown. cbn. 
+    have NEq: ot ≠ Tagged t.
+    { intros ->. specialize (Hneq' eq_refl). congruence. } 
+    move : NEq. by eapply retag_Some_local.
+Qed.
+
+Lemma bor_interp_retag_default σ_t σ_s c l ot T α' mut :
+  let pk : pointer_kind := RefPtr mut in
+  let pm := match mut with Mutable => Unique | Immutable => SharedReadOnly end in
+  let tk := match mut with Mutable => tk_unq | Immutable => tk_pub end in
+  retag σ_s.(sst) σ_s.(snp) σ_s.(scs) c l ot Default pk T = Some (Tagged σ_s.(snp), α', S σ_s.(snp)) →
+  c ∈ σ_s.(scs) →
+  (if mut is Immutable then is_freeze T else True) →
+  state_wf (mkState σ_t.(shp) α' σ_t.(scs) (S σ_t.(snp)) σ_t.(snc)) →   (* could remove that assumption *)
+  state_wf (mkState σ_s.(shp) α' σ_s.(scs) (S σ_s.(snp)) σ_s.(snc)) →   (* could remove that assumption *)
+  sc_rel (ScPtr l ot) (ScPtr l ot) -∗
+  bor_interp sc_rel σ_t σ_s ==∗ ∃ v_t v_s,
+  ⌜length v_t = tsize T⌝ ∗
+  ⌜length v_s = tsize T⌝ ∗
+  value_rel v_t v_s ∗
+  σ_t.(snp) $$ tk ∗
+  l ↦t∗[tk]{σ_t.(snp)} v_t ∗
+  l ↦s∗[tk]{σ_t.(snp)} v_s ∗
+  match mut with
+  | Mutable => True
+  | Immutable =>
+    sc_rel (ScPtr l (Tagged (σ_t.(snp)))) (ScPtr l (Tagged (σ_t.(snp))))
+  end ∗
+  bor_interp sc_rel (mkState σ_t.(shp) α' σ_t.(scs) (S σ_t.(snp)) σ_t.(snc)) (mkState σ_s.(shp) α' σ_s.(scs) (S σ_s.(snp)) σ_s.(snc)).
+Proof.
+  intros pk pm tk Hretag Hc_in Hfreeze Hwf'_t Hwf'_s.
+  iIntros "Hscrel Hbor". iDestruct "Hbor" as "(% & % & % & % & (Hc & Htag_auth & Htag_t_auth & Htag_s_auth) & #Hsrel & %Hcall_interp & %Htag_interp & %Hwf_s & %Hwf_t)".
+
+  iDestruct "Hscrel" as "[_ Hrel]".
+  iAssert (⌜untagged_or_public M_tag ot⌝)%I as %Hpub.
+  { iDestruct "Hrel" as "[[-> _] | (%t1 & %t2 & -> & -> & <- & Hpub)]"; first done.
+    iPoseProof (tkmap_lookup with "Htag_auth Hpub") as "%". done.
+  }
+  pose nt := (snp σ_t).
+
+  have Hin_dom := retag_Some_dom _ _ _ _ _ _ _ pk _ _ _ _ I Hretag.
+  iPoseProof (state_rel_dom_eq with "Hsrel") as "%Hdom_eq".
+  destruct (read_mem_is_Some l (tsize T) σ_s.(shp)) as [v_s Hv_s].
+  { setoid_rewrite (state_wf_dom _ Hwf_s). done. }
+  destruct (read_mem_is_Some l (tsize T) σ_t.(shp)) as [v_t Hv_t].
+  { rewrite Hdom_eq. setoid_rewrite (state_wf_dom _ Hwf_s). done. }
+  destruct (read_mem_values _ _ _ _ Hv_s) as [Hlen_s Hshp_s].
+  destruct (read_mem_values _ _ _ _ Hv_t) as [Hlen_t Hshp_t].
+
+  (* allocate resources *)
+  assert (M_tag !! nt = None) as Htag_none.
+  { destruct (M_tag !! nt) as [[tk' []] | ] eqn:Ht_some; last done.
+    apply Htag_interp in Ht_some as [Hcontra _]. lia. }
+  destruct Htag_interp as (Htag_interp & Ht_dom & Hs_dom).
+  iMod (tkmap_insert tk _ tt Htag_none with "Htag_auth") as "[Htag_auth Hnt]".
+  iMod (ghost_map_array_tag_insert _ _ v_t nt l with "Htag_t_auth") as "[Ht Htag_t_auth]".
+  { intros i Hi. destruct (M_t !! (nt, l +ₗ i)) eqn:Hmt; last done.
+    destruct (Ht_dom nt (l +ₗ i) ltac:(eauto)) as (? & ?); congruence. }
+  iMod (ghost_map_array_tag_insert _ _ v_s nt l with "Htag_s_auth") as "[Hs Htag_s_auth]".
+  { intros i Hi. destruct (M_s !! (nt, l +ₗ i)) eqn:Hmt; last done.
+    destruct (Hs_dom nt (l +ₗ i) ltac:(eauto)) as (? & ?); congruence. }
+  iMod (ghost_map_array_tag_tk _ _ _ _ tk with "Ht") as "Ht".
+  iMod (ghost_map_array_tag_tk _ _ _ _ tk with "Hs") as "Hs".
+  iModIntro.
+  iAssert (nt $$ tk ∗ if tk is tk_pub then nt $$ tk_pub else True)%I  with "[Hnt]" as "[$ Hpubt]".
+  { destruct tk; eauto. }
+  iExists v_t, v_s. iSplit; first done. iSplit; first done. iFrame "Ht Hs".
+
+  iAssert (⌜retag σ_t.(sst) σ_t.(snp) σ_t.(scs) c l ot Default pk T = Some (Tagged nt, α', S (σ_t.(snp)))⌝)%I as "%Hretag_t".
+  { iPoseProof (state_rel_calls_eq with "Hsrel") as "<-".
+    iPoseProof (state_rel_stacks_eq with "Hsrel") as "<-".
+    subst nt. iPoseProof (state_rel_snp_eq with "Hsrel") as "<-". done. }
+  (* proving the value relation *)
+  iAssert (value_rel v_t v_s)%I as "#Hvrel"; last iFrame "Hvrel".
+  { iApply big_sepL2_forall; iSplit; first (iPureIntro;lia).
+    iIntros (i sc_t sc_s) "%Hs_t %Hs_v".
+    assert (i < tsize T)%nat as Hi. { rewrite -Hlen_t. eapply lookup_lt_is_Some_1. eauto. }
+    assert (Hsome_target : is_Some (σ_t.(shp) !! (l +ₗ i))).
+    { rewrite Hshp_t; last done. apply lookup_lt_is_Some_2. by rewrite Hlen_t. }
+    iPoseProof (state_rel_pub_if_not_priv _ _ _ _ _ _ (l +ₗ i) with "[] Hsrel [Hrel]") as "Hpub"; first done.
+    { iPoseProof (state_rel_calls_eq with "Hsrel") as "%Hcall_eq".
+      iPoseProof (state_rel_stacks_eq with "Hsrel") as "%Hstack_eq".
+      iPureIntro. intros t Hpriv.
+      eapply (priv_loc_UB_retag_access_eq σ_s σ_t); eauto; done. }
+    iPoseProof (pub_loc_lookup with "[] Hpub") as "(%sc_t' & %sc_s' & %Hread_both & Hsc_rel)"; first done.
+    enough (sc_t = sc_t' ∧ sc_s = sc_s') by naive_solver.
+    move : Hs_t Hs_v Hread_both (Hshp_s i Hi) (Hshp_t i Hi).
+    by move => -> -> [-> ->] [= ->] [= ->].
+  }
+
+  iSplitL "Hpubt".
+  { destruct mut; first done. iSplitR; first done. iRight.
+    iExists (σ_t.(snp)), (σ_t.(snp)). do 3 (iSplitR; first done). done. }
+
+  (* re-establishing the interpretation *)
+  iExists M_call, (<[ nt := (tk, ()) ]> M_tag), (array_tag_map l nt v_t ∪ M_t), (array_tag_map l nt v_s ∪ M_s).
+  iFrame. iSplitL.
+  { (* state relation *)
+    rewrite /state_rel. simpl. iDestruct "Hsrel" as "(-> & %Hs_eq & -> & -> & -> & Hsrel)".
+    do 5 (iSplitL; first done). iIntros (l' Hsl').
+    iDestruct ("Hsrel" $! l' with "[//]") as "[Hpub | [%t' %Hpriv]]"; first (iLeft; iApply "Hpub").
+    iRight. iPureIntro. exists t'.
+    destruct Hpriv as (tk' & Hsome_tk' & Ht_l' & Htk'). exists tk'.
+    assert (t' ≠ nt). { intros ->. simplify_eq. }
+    rewrite lookup_insert_ne; last done.
+    split; first done. split; last done.
+    destruct Ht_l' as (sc0 & Ht_l'). exists sc0.
+    rewrite lookup_union_r; first done.
+    destruct (array_tag_map l nt v_t !! (t', l')) as [ a | ] eqn:Harr; last done.
+    specialize (array_tag_map_lookup1 l nt v_t t' l' ltac:(eauto)) as [Heq _]. congruence.
+  }
+  iSplitL.
+  { (* call interpretation. *)
+    iPureIntro. intros c' M' [Hc' HM']%Hcall_interp. split; first done.
+    intros t' S HS. simpl. specialize (HM' t' S HS) as (Ht' & Hprot).
+    split; first lia. intros l' Hl'.
+    specialize (Hprot l' Hl') as (s & pm' & Hs & Hit & Hpm').
+    specialize (retag_item_active_preserving _ _ _ _ _ _ _ _ _ _ _ _ Hretag_t l' s (Tagged t') c' pm' Hs Hc' Hit) as (s' & -> & Hin'). eauto.
+  }
+  iSplitL.
+  { (* tag interpretation. *)
+    iPoseProof (state_rel_get_pure with "Hsrel") as "%Hp".
+    destruct Hp as (Hsst & Hsnp & Hsnc & Hscs).
+    assert (∀l', M_t !! (nt, l') = None) as HMt_nt.
+    { intros l'. destruct (M_t !! (nt, l')) eqn:HM_t; last done. 
+      specialize (Ht_dom nt l' ltac:(eauto)) as (? & ?); congruence. }
+    assert (∀l', M_s !! (nt, l') = None) as HMs_nt.
+    { intros l'. destruct (M_s !! (nt, l')) eqn:HM_s; last done. 
+      specialize (Hs_dom nt l' ltac:(eauto)) as (? & ?); congruence. }
+    iPureIntro. split_and!.
+    { intros t tk'. rewrite lookup_insert_Some. intros [[<- [= <-]] | [Hneq Hsome_t]].
+      - cbn. split_and!; [lia | lia | | |].
+        + intros l' sc_t Ha%lookup_union_Some_l'; last done.
+          specialize (array_tag_map_lookup2 l nt v_t nt l' ltac:(eauto)) as [_ (i & Hi & ->)].
+          eapply retag_default_loc_controlled; [ done | done | lia | ].
+          move : Ha. rewrite array_tag_map_lookup_Some; last done. move => <-. apply Hshp_t. lia.
+        + intros l' sc_s Ha%lookup_union_Some_l'; last done.
+          specialize (array_tag_map_lookup2 l nt v_s nt l' ltac:(eauto)) as [_ (i & Hi & ->)].
+          subst nt. rewrite -Hsnp. eapply retag_default_loc_controlled; [ done | done | lia | ].
+          move : Ha. rewrite array_tag_map_lookup_Some; last done. move => <-. apply Hshp_s. lia.
+        + apply dom_agree_on_tag_union. { apply dom_agree_on_tag_array_tag_map. lia. } 
+          apply dom_agree_on_tag_not_elem; done.
+      - cbn. 
+        specialize (Htag_interp t tk' Hsome_t) as (Ht_t & Ht_s & Hcontrolled_t & Hcontrolled_s & Hagree). 
+        split_and!; [ lia | lia | | | ].
+        + intros l' sc_t Ha. rewrite lookup_union_r in Ha; last by apply array_tag_map_lookup_None.
+          apply Hcontrolled_t in Ha. 
+          eapply retag_default_loc_controlled'; [done | done | done | | done | done | done].
+          intros <-. destruct tk'; [ done | | ]; move : Hsome_t Hpub; congruence.
+        + intros l' sc_s Ha. rewrite lookup_union_r in Ha; last by apply array_tag_map_lookup_None.
+          apply Hcontrolled_s in Ha. 
+          eapply retag_default_loc_controlled'; [done | done | done | | congruence | done | done].
+          intros <-. destruct tk'; [ done | | ]; move : Hsome_t Hpub; congruence.
+        + apply dom_agree_on_tag_union; last done. 
+          apply dom_agree_on_tag_not_elem; apply array_tag_map_lookup_None; done. 
+    }
+    { intros t l'. 
+      rewrite lookup_union_is_Some lookup_insert_is_Some'. intros [[-> _]%array_tag_map_lookup2 | H%Ht_dom]; eauto. } 
+    { intros t l'.
+      rewrite lookup_union_is_Some lookup_insert_is_Some'. intros [[-> _]%array_tag_map_lookup2 | H%Hs_dom]; eauto. }
+  } 
+  done.
+Qed.
+
 (* TODO: for Mutable, this is currently not particularly useful, since reads are UB when the tag is not there.
   Instead, need a mechanism for "deferred observations" or such
 *)
 Lemma sim_retag_default mut T l_t l_s c ot π Φ :
-  (0 < tsize T)%nat → (* TODO: check if we need that condition *)
+  (0 < tsize T)%nat → (* for convenience: makes the proof easier *)
   let pk : pointer_kind := RefPtr mut in
   let pm := match mut with Mutable => Unique | Immutable => SharedReadOnly end in
+  let tk := match mut with Mutable => tk_unq | Immutable => tk_pub end in
   (if mut is Immutable then is_freeze T else True) →
   sc_rel (ScPtr l_t ot) (ScPtr l_s ot) -∗
   (∀ nt v_t v_s,
-    let tk := match mut with Mutable => tk_unq | Immutable => tk_pub end in
     ⌜length v_t = tsize T⌝ -∗ ⌜length v_s = tsize T⌝ -∗
     value_rel v_t v_s -∗  (* as the pointers were public before *)
     nt $$ tk -∗
@@ -1493,7 +1992,43 @@ Lemma sim_retag_default mut T l_t l_s c ot π Φ :
     #[ScPtr l_t (Tagged nt)] ⪯{π, Ω} #[ScPtr l_s (Tagged nt)] [{ Φ }]) -∗
   Retag #[ScPtr l_t ot] #[ScCallId c] pk T Default ⪯{π, Ω} Retag #[ScPtr l_s ot] #[ScCallId c] pk T Default [{ Φ }].
 Proof.
-Admitted.
+  intros Hsize pk pm tk Hmut. iIntros "#Hscrel Hsim".
+  iApply sim_lift_head_step_both. iIntros (??????) "((HP_t & HP_s & Hbor) & %Hthread & %Hsafe)".
+  (* exploit source to gain knowledge about stacks & that c is a valid id *)
+  specialize (pool_safe_irred _ _ _ _ _ _ _ Hsafe Hthread ltac:(done)) as (c' & ot' & l' & [= <- <-] & [= <-] & Hc_active & Hretag_some_s).
+  iPoseProof "Hscrel" as "(-> & _)".
+  iPoseProof (bor_interp_get_pure with "Hbor") as "%Hp".
+  have Hretag_some_t : is_Some (retag σ_t.(sst) σ_t.(snp) σ_t.(scs) c l_s ot Default pk T).
+  { destruct Hp as (<- & <- & _ & <- & _). done. }
+  iModIntro. iSplitR.
+  { iPureIntro.
+    destruct Hretag_some_t as ([[] ] & Hretag_some_t).
+    do 3 eexists. eapply retag_head_step'; last done.
+    destruct Hp as (_ & _ & _ & <- & _). done.
+  }
+  iIntros (e_t' efs_t σ_t') "%Hhead_t".
+  specialize (head_retag_inv _ _ _ _ _ _ _ _ _ _ _ Hhead_t) as (nt & α' & nxtp' & Hretag_t & -> & -> & -> & Hc).
+  have Hretag_s : retag σ_s.(sst) σ_s.(snp) σ_s.(scs) c l_s ot Default pk T = Some (nt, α', nxtp').
+  { destruct Hp as (-> & -> & _ & -> & _). done. }
+  assert (Hhead_s : head_step P_s (Retag #[ScPtr l_s ot] #[ScCallId c] pk T Default) σ_s #[ScPtr l_s nt]%E (mkState (shp σ_s) α' (scs σ_s) nxtp' (snc σ_s)) []).
+  { eapply retag_head_step'; done. }
+  specialize (retag_change_ref_NZST _ _ _ _ _ _ _ _ _ _ _ _ Hsize Hretag_s) as [-> ->].
+
+  iPoseProof (bor_interp_get_state_wf with "Hbor") as "[%Hwf_t %Hwf_s]".
+  iMod (bor_interp_retag_default _ _ _ _ _ _ _ _ Hretag_s ltac:(done) with "Hscrel Hbor") as
+    (v_t v_s) "(%Hlen_t & %Hlen_s & Hval & Htag & Ht & Hs & Hpub & Hbor)"; first done.
+  { destruct Hp as (_ & <- & _). eapply head_step_wf; eauto. }
+  { eapply head_step_wf; eauto. }
+  iModIntro.
+
+  iExists #[ScPtr l_s (Tagged σ_s.(snp))]%E, [], (mkState σ_s.(shp) α' σ_s.(scs) (S σ_s.(snp)) σ_s.(snc)).
+  iSplitR; first done.
+  destruct Hp as (_ & -> & _).
+  iFrame "Hbor HP_t HP_s".
+  iSplitL; last done.
+  iApply ("Hsim" with "[] [] Hval Htag Ht Hs Hpub"); [done | done | ..].
+Qed.
+
 
 Fixpoint seq_loc_set (l : loc) (n : nat) : gset loc :=
   match n with
@@ -1522,24 +2057,165 @@ Lemma sim_retag_fnentry mut T l_t l_s c M ot π Φ :
 Proof.
 Admitted.
 
-Lemma sim_initcall π Φ :
+Lemma bor_interp_init_call σ_t σ_s :
+  bor_interp sc_rel σ_t σ_s ==∗
+  σ_t.(snc) @@ ∅ ∗
+  bor_interp sc_rel
+    (mkState σ_t.(shp) σ_t.(sst) ({[ σ_t.(snc) ]} ∪ σ_t.(scs)) σ_t.(snp) (S σ_t.(snc)))
+    (mkState σ_s.(shp) σ_s.(sst) ({[ σ_s.(snc) ]} ∪ σ_s.(scs)) σ_s.(snp) (S σ_s.(snc))).
+Proof.
+  iIntros "(% & % & % & % & (Hc & Htag_auth & Htag_t_auth & Htag_s_auth) & #Hsrel & %Hcall_interp & %Htag_interp & %Hwf_s & %Hwf_t)".
+  iPoseProof (state_rel_snc_eq with "Hsrel") as "%Hsnc_eq".
+  assert (M_call !! σ_t.(snc) = None) as Hfresh.
+  { destruct (M_call !! σ_t.(snc)) as [ M' | ] eqn:HM'; last done. apply Hcall_interp in HM' as (Hin & _).
+    apply Hwf_t in Hin. lia. }
+  iMod (ghost_map_insert σ_t.(snc) ∅ Hfresh with "Hc") as "[Hc Hcall]".
+  iModIntro. iFrame "Hcall".
+  iExists (<[σ_t.(snc) := ∅]> M_call), M_tag, M_t, M_s. iFrame.
+  iSplitL.
+  { iDestruct "Hsrel" as "(H1 & H2 & H3 & H4 & %H5 & H6)". rewrite /state_rel. simpl.
+    iFrame "H1 H2 H3".
+    iSplitR. { iPureIntro. lia. }
+    iSplitR. { rewrite H5 Hsnc_eq. done. }
+    iIntros (l Hl). iDestruct ("H6" $! l with "[//]") as "[Hpub | (%t & %Hpriv)]".
+    - iLeft. iApply "Hpub".
+    - iRight. iPureIntro. exists t.
+      destruct Hpriv as (tk & Htk & Hs & [-> | [-> (c' & Hin)]]).
+      { exists tk_local. split_and!; eauto. }
+      exists tk_unq. split_and!; [done.. | ]. right. split; first done.
+      exists c'. destruct Hin as (M' & HM' & Hin). exists M'.
+      split; last done. apply lookup_insert_Some. right. split; last done.
+      apply Hcall_interp in HM' as (Hwf_tag & _).
+      specialize (state_wf_cid_agree _ Hwf_t _ Hwf_tag). lia.
+  }
+  iSplitL.
+  { iPureIntro. intros c M'. simpl. rewrite lookup_insert_Some. intros [(<- & <-) | [Hneq Hsome]].
+    - split; first set_solver. intros ? ?. rewrite lookup_empty. congruence.
+    - rewrite elem_of_union. apply Hcall_interp in Hsome as [Hin Ha]. split; [by eauto | done].
+  }
+  iSplitL. { iPureIntro. apply Htag_interp. }
+  iSplitL. { iPureIntro. destruct Hwf_s. constructor; simpl; try done.
+    - intros l stk Hstk. apply state_wf_stack_item in Hstk.
+      destruct Hstk as [Hstk ?]. split; last done. intros i Hi. specialize (Hstk i Hi).
+      destruct tg, protector; naive_solver.
+    - intros c. rewrite elem_of_union elem_of_singleton. intros [-> | Hin%state_wf_cid_agree]; lia.
+  }
+  (* TODO: duplicated proof *)
+  iPureIntro. destruct Hwf_t. constructor; simpl; try done.
+  - intros l stk Hstk. apply state_wf_stack_item in Hstk.
+    destruct Hstk as [Hstk ?]. split; last done. intros i Hi. specialize (Hstk i Hi).
+    destruct tg, protector; naive_solver.
+  - intros c. rewrite elem_of_union elem_of_singleton. intros [-> | Hin%state_wf_cid_agree]; lia.
+Qed.
+
+Lemma head_init_call_inv (P : prog) e' σ σ' efs :
+  head_step P InitCall σ e' σ' efs →
+  ∃ c,
+    c = σ.(snc) ∧
+    efs = [] ∧
+    e' = (#[ScCallId c])%E ∧
+    σ' = (mkState σ.(shp) σ.(sst) ({[ σ.(snc) ]} ∪ σ.(scs)) σ.(snp) (S σ.(snc))).
+Proof. intros Hhead. inv_head_step. eauto. Qed.
+
+Lemma sim_init_call π Φ :
   (∀ c, c @@ ∅ -∗
     #[ScCallId c] ⪯{π, Ω} #[ScCallId c] [{ Φ }]) -∗
   InitCall ⪯{π, Ω} InitCall [{ Φ }].
 Proof.
-Admitted.
+  iIntros "Hsim". iApply sim_lift_head_step_both. iIntros (??????) "((HP_t & HP_s & Hbor) & _ & _)".
+  iPoseProof (bor_interp_get_pure with "Hbor") as "%Hp".
+  iMod (bor_interp_init_call with "Hbor") as "[Hc Hbor]". iModIntro.
+  iSplitR.
+  { iPureIntro. do 3 eexists. eapply init_call_head_step. }
+  iIntros (e_t' efs_t σ_t') "%Hhead".
+  specialize (head_init_call_inv _ _ _ _ _ Hhead) as (c & Heqc & -> & -> & ->).
+  iModIntro. iExists (#[ScCallId σ_s.(snc)])%E, [], (mkState σ_s.(shp) σ_s.(sst) ({[ σ_s.(snc) ]} ∪ σ_s.(scs)) σ_s.(snp) (S σ_s.(snc))).
+  iSplitR. { iPureIntro. eapply init_call_head_step. }
+  iSplitR "Hsim Hc"; first last.
+  { iSplitL; last done. destruct Hp as (_ & _ & Heqc' & _). rewrite Heqc Heqc'. by iApply "Hsim". }
+  iFrame.
+Qed.
 
-(* TODO: should we require that M = ∅ here and provide lemmas that allow to empty this?
-  That is what the original formalization does, but I don't think we will need it..
-*)
-Lemma sim_endcall c M π Φ :
-  c @@ M -∗
+Lemma bor_interp_end_call c σ_t σ_s :
+  bor_interp sc_rel σ_t σ_s -∗
+  c @@ ∅ ==∗ (* we need it to be empty to avoid tripping private locations *)
+  ⌜c ∈ σ_t.(scs) ∧ c ∈ σ_s.(scs)⌝ ∗ bor_interp sc_rel (state_upd_calls (.∖ {[ c ]}) σ_t) (state_upd_calls (.∖ {[ c ]}) σ_s).
+Proof.
+  iIntros "(% & % & % & % & (Hc & Htag_auth & Htag_t_auth & Htag_s_auth) & #Hsrel & %Hcall_interp & %Htag_interp & %Hwf_s & %Hwf_t) Hcall".
+  iPoseProof (ghost_map_lookup with "Hc Hcall") as "%Hlookup".
+  iMod (ghost_map_delete with "Hc Hcall") as "Hc". iModIntro.
+  iPoseProof (state_rel_calls_eq with "Hsrel") as "->".
+  iSplitR.
+  { destruct (Hcall_interp _ _ Hlookup) as (? & _). done. }
+  iExists (delete c M_call), M_tag, M_t, M_s. iFrame.
+  iSplitL "Hsrel".
+  { iDestruct "Hsrel" as "(H1 & H2 & H3 & H4 & %H5 & H6)". rewrite /state_rel. cbn.
+    iFrame "H1 H2 H3 H4".
+    iSplitR. { rewrite H5. done. }
+    iIntros (l Hl). iDestruct ("H6" $! l with "[//]") as "[Hpub | (%t & %Hpriv)]".
+    - iLeft. iApply "Hpub".
+    - iRight. iPureIntro. exists t.
+      destruct Hpriv as (tk & Htk & Hs & [-> | [-> (c' & Hin)]]).
+      { exists tk_local. split_and!; eauto. }
+      exists tk_unq. split_and!; [done.. | ]. right. split; first done.
+      exists c'. destruct Hin as (M' & HM' & Hin). exists M'.
+      assert (c ≠ c') as Hneq.
+      { intros <-. simplify_eq. destruct Hin as (L & Hsome & _).
+        rewrite lookup_empty in Hsome. done.
+      }
+      rewrite lookup_delete_ne; last done. done.
+  }
+  iSplitL.
+  { iPureIntro. by apply call_set_interp_remove. }
+  iSplitL.
+  { iPureIntro. apply Htag_interp. }
+  iSplitL.
+  { iPureIntro. destruct Hwf_s. constructor; [done.. | ].
+    intros c'. cbn. rewrite elem_of_difference. intros [Hin _]. eauto. }
+  iPureIntro. destruct Hwf_t. constructor; [done.. | ].
+  intros c'. cbn. rewrite elem_of_difference. intros [Hin _]. eauto.
+Qed.
+
+Lemma head_end_call_inv (P : prog) e' σ σ' efs c :
+  head_step P (EndCall #[ScCallId c]) σ e' σ' efs →
+  c ∈ σ.(scs) ∧
+  efs = [] ∧
+  e' = (#[☠])%E ∧
+  σ' = state_upd_calls (.∖ {[ c ]}) σ.
+Proof. intros Hhead. inv_head_step. eauto. Qed.
+
+Lemma sim_endcall c π Φ :
+  c @@ ∅ -∗ (* needs to be empty so we don't trip private locations *)
   #[☠] ⪯{π, Ω} #[☠] [{ Φ }] -∗
   EndCall #[ScCallId c] ⪯{π, Ω} EndCall #[ScCallId c] [{ Φ }].
 Proof.
+  iIntros "Hcall Hsim". iApply sim_lift_head_step_both. iIntros (??????) "((HP_t & HP_s & Hbor) & _ & _)".
+  iMod (bor_interp_end_call with "Hbor Hcall") as "[%Hc_in Hbor]". iModIntro.
+  iSplitR.
+  { iPureIntro. do 3 eexists. eapply end_call_head_step. apply Hc_in. }
+  iIntros (e_t' efs_t σ_t') "%Hhead".
+  specialize (head_end_call_inv _ _ _ _ _ _ Hhead) as (_ & -> & -> & ->).
+  iModIntro. iExists (#[☠])%E, [], (state_upd_calls (.∖ {[ c ]}) σ_s).
+  iSplitR. { iPureIntro. eapply end_call_head_step. apply Hc_in. }
+  iSplitR "Hsim"; first last.
+  { iFrame "Hsim". done. }
+  iFrame.
+Qed.
+
+(* TODO: maybe formulate that with [update_si] instead *)
+Lemma sim_protected_unprotect S M l c t tk sc_t sc_s  π Φ e_t e_s :
+  l ∈ S →
+  M !! t = Some S →
+  c @@ M -∗
+  l ↦t[tk]{t} sc_t -∗
+  l ↦s[tk]{t} sc_s -∗
+  sc_rel sc_t sc_s -∗
+  (c @@ (<[t := S ∖ {[ l ]} ]> M) → e_t ⪯{π, Ω} e_s [{ Φ }]) -∗
+  e_t ⪯{π, Ω} e_s [{ Φ }].
+Proof.
 Admitted.
 
-Lemma sim_call fn r_t r_s π Φ :
+Lemma sim_call fn (r_t r_s : result) π Φ :
   Ω r_t r_s -∗
   (∀ r_t r_s : result, Ω r_t r_s -∗ Φ (of_result r_t) (of_result r_s)) -∗
   Call #[ScFnPtr fn] r_t ⪯{π, Ω} Call #[ScFnPtr fn] r_s [{ Φ }].
